src/MicroSail/Symbolic/Sound.v
@@ -314,6 +314,11 @@ Module Soundness
       scmut_wp sm1 POST s__sc \/ scmut_wp sm2 POST s__sc.
     Proof. unfold scmut_wp, scmut_angelic_binary; cbn; intuition. Qed.
 
+    Lemma scmut_wp_state {Γ1 Γ2 A} (f : SCState Γ1 -> A * SCState Γ2) (POST : A -> SCState Γ2 -> Prop) :
+      forall (s1 : SCState Γ1),
+        scmut_wp (scmut_state f) POST s1 <-> POST (fst (f s1)) (snd (f s1)).
+    Proof. intros s1. cbn. now destruct (f s1); cbn. Qed.
+
   End SemiConcreteWP.
 
   Module TwoPointOSoundness.
@@ -585,6 +590,18 @@ Module Soundness
       now apply dmut_arrow_dcl_specialize.
     Qed.
 
+    Lemma dmut_sub_arrow_dcl {AT A BT B} `{InstLaws AT A, InstLaws BT B} {Γ2 Γ3 Σ0} (d : DynamicMutator Γ2 Γ3 BT Σ0) (d_dcl : dmut_dcl d) :
+      dmut_arrow_dcl (fun (Σ2 : LCtx) (ζ02 : Sub Σ0 Σ2) (_ : AT Σ2) => dmut_sub ζ02 d).
+    Proof. intros until Q; intros PQ. rewrite ?dmut_wp_sub. eapply d_dcl; eauto. Qed.
+
+    Lemma dmut_pure_arrow_dcl {AT A} `{InstLaws AT A} {Γ Σ0} :
+      dmut_arrow_dcl (fun Σ1 (ζ01 : Sub Σ0 Σ1) (a1 : AT Σ1) => dmut_pure (Γ := Γ) a1).
+    Proof.
+      intros until Q; intros PQ. cbn.
+      intros HP. apply PQ. revert HP.
+      rewrite ?inst_subst. intuition.
+    Qed.
+
     Lemma dmut_wp_bind_left {AT A BT B} `{InstLaws AT A, InstLaws BT B} {Γ1 Γ2 Γ3 Σ0 Σ1}
           (d1 : DynamicMutator Γ1 Γ2 AT Σ0) (d2 : DynamicMutator Γ2 Γ3 BT Σ0) (d2_dcl : dmut_dcl d2)
           (ζ01 : Sub Σ0 Σ1) (pc1 : PathCondition Σ1) (s1 : SymbolicState Γ1 Σ1) (ι1 : SymInstance Σ1)
@@ -598,9 +615,9 @@ Module Soundness
         intros _ sc3; now rewrite dmut_wp_pure, ?inst_lift.
       apply dmut_pure_dcl.
       apply dmut_bind_right_arrow_dcl.
-      admit.
-      admit.
-    Admitted.
+      now apply dmut_sub_arrow_dcl.
+      apply dmut_pure_arrow_dcl.
+    Qed.
 
     Lemma dmut_wp_state {AT A} `{Inst AT A, Subst AT} {Γ1 Γ2 Σ1 Σ2} (f : forall Σ2, Sub Σ1 Σ2 -> SymbolicState Γ1 Σ2 -> Pair AT (SymbolicState Γ2) Σ2)
           (pc2 : PathCondition Σ2) (s12 : SymbolicState Γ1 Σ2) (ζ12 : Sub Σ1 Σ2) (ι2 : SymInstance Σ2) (F : string -> Prop) (Q : A -> SCState Γ2 -> Prop) :
@@ -652,29 +669,37 @@ Module Soundness
         unfold sub_comp. now rewrite inst_subst, inst_sub_wk1.
     Qed.
 
-    Lemma dmut_wp_angelic_list {AT A D} `{Inst AT A, Subst AT} {Γ1 Γ2 Σ} (func msg : string) (data : D)
-          (ds : list (DynamicMutator Γ1 Γ2 AT Σ)) Σ1 (ζ01 : Sub Σ Σ1) (pc1 : PathCondition Σ1)
-          (s11 : SymbolicState Γ1 Σ1) (ι1 : SymInstance Σ1) :
-      forall F P,
-        dmut_wp (dmut_angelic_list func msg data ds) ζ01 pc1 s11 ι1 F P <->
-        (exists d, List.In d ds /\ dmut_wp d ζ01 pc1 s11 ι1 F P).
+    Lemma dmut_wp_angelic_list {AT A D} `{InstLaws AT A} {Γ Σ} (func msg : string) (data : D)
+      (xs : List AT Σ) Σ1 (ζ01 : Sub Σ Σ1) (pc1 : PathCondition Σ1) (s11 : SymbolicState Γ Σ1) (ι1 : SymInstance Σ1)
+      (F : string -> Prop) (P : A -> SCState Γ -> Prop) :
+      dmut_wp (dmut_angelic_list func msg data xs) ζ01 pc1 s11 ι1 F P <->
+      exists x : AT _, List.In x xs /\ P (inst (inst ι1 ζ01) x) (inst ι1 s11).
     Proof.
-      intros F P.
-      induction ds; cbn - [dmut_wp].
+      induction xs; cbn - [dmut_wp].
       - rewrite dmut_wp_fail. split. admit.
         intros []; intuition.
-      - destruct ds; cbn - [dmut_wp] in *.
-        + rewrite dmut_wp_fail in IHds.
-          destruct IHds. split; intros; destruct_conjs.
+      - destruct xs; cbn - [dmut_wp] in *.
+        + rewrite dmut_wp_fail in IHxs.
+          rewrite dmut_wp_pure.
+          destruct IHxs. split; intros; destruct_conjs.
           exists a. intuition.
           intuition.
-        + admit.
+        + rewrite dmut_wp_angelic_binary, dmut_wp_pure.
+          split. intros [Hwp|Hwp].
+          * exists a. split; auto.
+          * apply IHxs in Hwp. destruct Hwp as [x [Hwp HP]].
+            exists x. split; auto.
+          * intros [x [Hwp HP]].
+            destruct Hwp as [Hwp|Hwp]. subst. left. auto.
+            destruct Hwp as [Hwp|Hwp]. subst.
+            right. apply IHxs. exists x. split; auto.
+            right. apply IHxs. exists x. split; auto.
     Admitted.
 
-    Lemma dmut_wp_demonic_finite {X AT A} `{finite.Finite X, Subst AT, Inst AT A} {Γ Σ Σ1}
-      (k : X -> DynamicMutator Γ Γ AT Σ) (k_dcl : forall x, dmut_dcl (k x))
-      (ζ01 : Sub Σ Σ1) (pc1 : PathCondition Σ1) (s1 : SymbolicState Γ Σ1) (ι1 : SymInstance Σ1)
-      (F : string -> Prop) (P : A -> SCState Γ -> Prop) :
+    Lemma dmut_wp_demonic_finite {X AT A} `{finite.Finite X, Subst AT, Inst AT A} {Γ1 Γ2 Σ Σ1}
+      (k : X -> DynamicMutator Γ1 Γ2 AT Σ) (k_dcl : forall x, dmut_dcl (k x))
+      (ζ01 : Sub Σ Σ1) (pc1 : PathCondition Σ1) (s1 : SymbolicState Γ1 Σ1) (ι1 : SymInstance Σ1)
+      (F : string -> Prop) (P : A -> SCState Γ2 -> Prop) :
       dmut_wp (dmut_demonic_finite X k) ζ01 pc1 s1 ι1 F P <->
       (forall x : X, dmut_wp (k x) ζ01 pc1 s1 ι1 F P).
     Proof.
@@ -747,8 +772,10 @@ Module Soundness
       dmut_dcl (dmut_bind_left d1 d2).
     Proof.
       unfold dmut_bind_left. apply dmut_bind_dcl; auto.
-      apply dmut_bind_right_arrow_dcl. admit. admit.
-    Admitted.
+      apply dmut_bind_right_arrow_dcl.
+      now apply dmut_sub_arrow_dcl.
+      apply dmut_pure_arrow_dcl.
+    Qed.
 
     Lemma dmut_demonic_binary_dcl {Γ1 Γ2 AT A Σ0} `{Inst AT A, Subst AT} (d1 d2 : DynamicMutator Γ1 Γ2 AT Σ0) (d1_dcl : dmut_dcl d1) (d2_dcl : dmut_dcl d2) :
       dmut_dcl (dmut_demonic_binary d1 d2).
@@ -785,6 +812,15 @@ Module Soundness
     Qed.
     Local Hint Resolve dmut_state_dcl : core.
 
+    Lemma dmut_put_heap_dcl {Γ Σ} (h : SymbolicHeap Σ) :
+      dmut_dcl (dmut_put_heap (Γ := Γ) h).
+    Proof.
+      apply dmut_state_dcl. destruct s1 as [δ h1], s2 as [δ2 h2].
+      cbn. intros ? ? -> Heqs Heqζ. inversion Heqs.
+      f_equal. f_equal. rewrite ?inst_subst. intuition.
+    Qed.
+    Local Hint Resolve dmut_put_heap_dcl : core.
+
     Lemma dmut_pop_local_dcl {Γ x σ Σ} :
       dmut_dcl (@dmut_pop_local Γ x σ Σ).
     Proof.
@@ -800,51 +836,51 @@ Module Soundness
       dmut_dcl (Γ1 := Γ1) (Γ2 := Γ2) (Σ0 := Σ) dmut_block.
     Proof. now unfold dmut_dcl, dmut_block. Qed.
 
-    Lemma dmut_demonic_list_dcl {AT A} `{Subst AT, Inst AT A} {Γ1 Γ2 Σ} (l : list (DynamicMutator Γ1 Γ2 AT Σ))
-      (l_dcl : forall d, List.In d l -> dmut_dcl d) :
-      dmut_dcl (dmut_demonic_list l).
-    Proof.
-      induction l; cbn.
-      - apply dmut_block_dcl.
-      - destruct l.
-        + apply l_dcl. now left.
-        + apply dmut_demonic_binary_dcl.
-          apply l_dcl. now left.
-          apply IHl. intros d' dIn'.
-          apply l_dcl. now right.
-    Qed.
+    (* Lemma dmut_demonic_list_dcl {AT A} `{Subst AT, Inst AT A} {Γ1 Γ2 Σ} (l : list (DynamicMutator Γ1 Γ2 AT Σ)) *)
+    (*   (l_dcl : forall d, List.In d l -> dmut_dcl d) : *)
+    (*   dmut_dcl (dmut_demonic_list l). *)
+    (* Proof. *)
+    (*   induction l; cbn. *)
+    (*   - apply dmut_block_dcl. *)
+    (*   - destruct l. *)
+    (*     + apply l_dcl. now left. *)
+    (*     + apply dmut_demonic_binary_dcl. *)
+    (*       apply l_dcl. now left. *)
+    (*       apply IHl. intros d' dIn'. *)
+    (*       apply l_dcl. now right. *)
+    (* Qed. *)
 
-    Lemma dmut_angelic_list_dcl {AT A D} `{Subst AT, Inst AT A} {Γ1 Γ2 Σ} func msg (data : D) (l : list (DynamicMutator Γ1 Γ2 AT Σ))
-      (l_dcl : forall d, List.In d l -> dmut_dcl d) :
-      dmut_dcl (dmut_angelic_list func msg data l).
-    Proof.
-      induction l; cbn.
-      - apply dmut_fail_dcl.
-      - destruct l.
-        + apply l_dcl. now left.
-        + apply dmut_angelic_binary_dcl.
-          apply l_dcl. now left.
-          apply IHl. intros d' dIn'.
-          apply l_dcl. now right.
-    Qed.
+    (* Lemma dmut_angelic_list_dcl {AT A D} `{Subst AT, Inst AT A} {Γ1 Γ2 Σ} func msg (data : D) (l : list (DynamicMutator Γ1 Γ2 AT Σ)) *)
+    (*   (l_dcl : forall d, List.In d l -> dmut_dcl d) : *)
+    (*   dmut_dcl (dmut_angelic_list func msg data l). *)
+    (* Proof. *)
+    (*   induction l; cbn. *)
+    (*   - apply dmut_fail_dcl. *)
+    (*   - destruct l. *)
+    (*     + apply l_dcl. now left. *)
+    (*     + apply dmut_angelic_binary_dcl. *)
+    (*       apply l_dcl. now left. *)
+    (*       apply IHl. intros d' dIn'. *)
+    (*       apply l_dcl. now right. *)
+    (* Qed. *)
 
-    Lemma dmut_demonic_finite_dcl {F AT A} `{finite.Finite F, Subst AT, Inst AT A} {Γ Σ}
-      (k : F -> DynamicMutator Γ Γ AT Σ) (k_dcl : forall x, dmut_dcl (k x)) :
-      dmut_dcl (dmut_demonic_finite F k).
-    Proof.
-      unfold dmut_demonic_finite. apply dmut_demonic_list_dcl.
-      intros d. rewrite List.in_map_iff.
-      intros [x [? xIn]]. subst d. apply k_dcl.
-    Qed.
+    (* Lemma dmut_demonic_finite_dcl {F AT A} `{finite.Finite F, Subst AT, Inst AT A} {Γ Σ} *)
+    (*   (k : F -> DynamicMutator Γ Γ AT Σ) (k_dcl : forall x, dmut_dcl (k x)) : *)
+    (*   dmut_dcl (dmut_demonic_finite F k). *)
+    (* Proof. *)
+    (*   unfold dmut_demonic_finite. apply dmut_demonic_list_dcl. *)
+    (*   intros d. rewrite List.in_map_iff. *)
+    (*   intros [x [? xIn]]. subst d. apply k_dcl. *)
+    (* Qed. *)
 
-    Lemma dmut_angelic_finite_dcl {F AT A} `{finite.Finite F, Subst AT, Inst AT A} {Γ Σ}
-      (k : F -> DynamicMutator Γ Γ AT Σ) (k_dcl : forall x, dmut_dcl (k x)) :
-      dmut_dcl (dmut_angelic_finite F k).
-    Proof.
-      unfold dmut_angelic_finite. apply dmut_angelic_list_dcl.
-      intros d. rewrite List.in_map_iff.
-      intros [x [? xIn]]. subst d. apply k_dcl.
-    Qed.
+    (* Lemma dmut_angelic_finite_dcl {F AT A} `{finite.Finite F, Subst AT, Inst AT A} {Γ Σ} *)
+    (*   (k : F -> DynamicMutator Γ Γ AT Σ) (k_dcl : forall x, dmut_dcl (k x)) : *)
+    (*   dmut_dcl (dmut_angelic_finite F k). *)
+    (* Proof. *)
+    (*   unfold dmut_angelic_finite. apply dmut_angelic_list_dcl. *)
+    (*   intros d. rewrite List.in_map_iff. *)
+    (*   intros [x [? xIn]]. subst d. apply k_dcl. *)
+    (* Qed. *)
 
     Lemma dmut_wp_assume_formula {Γ Σ1 Σ2} (ζ12 : Sub Σ1 Σ2) (pc2 : PathCondition Σ2) (fml : Formula Σ1) (s2 : SymbolicState Γ Σ2)
           (ι2 : SymInstance Σ2) (F : string -> Prop) P :
@@ -861,6 +897,24 @@ Module Soundness
         revert H5. rewrite ?inst_subst.
         rewrite H3, H4. apply PQ.
     Qed.
+
+    Lemma dmut_wp_assume_formulas {Γ Σ1 Σ2} (ζ12 : Sub Σ1 Σ2) (pc2 : PathCondition Σ2) (fmls : list (Formula Σ1)) (s2 : SymbolicState Γ Σ2)
+      (ι2 : SymInstance Σ2) (Hpc2 : instpc ι2 pc2) (F : string -> Prop) P (HF : forall e, F e <-> False) :
+      dmut_wp (dmut_assume_formulas fmls) ζ12 pc2 s2 ι2 F P <->
+      (instpc (inst ι2 ζ12) fmls -> P tt (inst ι2 s2)).
+    Proof.
+      unfold dmut_assume_formulas. revert s2.
+      induction fmls; cbn [List.fold_right]; intros s2.
+      - rewrite dmut_wp_pure. cbn. intuition.
+        apply H. constructor.
+      - rewrite dmut_wp_bind_right; auto.
+        rewrite dmut_wp_assume_formula; auto.
+        rewrite IHfmls.
+        rewrite inst_pathcondition_cons.
+        rewrite inst_lift.
+        intuition.
+        admit.
+    Admitted.
 
     Lemma dmut_assume_formula_dcl {Γ Σ} (fml : Formula Σ) :
       dmut_dcl (Γ1 := Γ) (dmut_assume_formula fml).
@@ -915,7 +969,7 @@ Module Soundness
     Proof. Admitted.
 
     Lemma dmut_wp_match_enum {AT A E} `{InstLaws AT A} {Γ1 Γ2 Σ1} (t : Term Σ1 (ty_enum E))
-      (d : 𝑬𝑲 E -> DynamicMutator Γ1 Γ2 AT Σ1)
+      (d : 𝑬𝑲 E -> DynamicMutator Γ1 Γ2 AT Σ1) (d_dcl : forall x, dmut_dcl (d x))
       Σ2 (ζ12 : Sub Σ1 Σ2) pc2 s2 ι2 F P :
       instpc ι2 pc2 ->
       dmut_wp (dmut_match_enum t d) ζ12 pc2 s2 ι2 F P <->
@@ -924,8 +978,24 @@ Module Soundness
       intros Hpc2. unfold dmut_match_enum. cbn.
       destruct (term_get_lit_spec (subst (T := fun Σ => Term Σ (ty_enum E)) ζ12 t)) as [k Heqιs|]; cbn [Lit] in *.
       - fold_dmut_wp. specialize (Heqιs ι2). rewrite inst_subst in Heqιs. now rewrite Heqιs.
-      - fold_dmut_wp. admit.
-    Admitted.
+      - fold_dmut_wp. rewrite dmut_wp_demonic_finite. split; intros Hwp.
+        + specialize (Hwp (inst (T := fun Σ => Term Σ _) (inst ι2 ζ12) t)).
+          rewrite dmut_wp_bind_right, dmut_wp_assume_formula, dmut_wp_sub in Hwp; auto.
+          rewrite sub_comp_id_right, inst_sub_id in Hwp. cbn in Hwp.
+          inster Hwp by now rewrite inst_subst. revert Hwp.
+          eapply d_dcl; rewrite ?inst_sub_id, ?inst_lift; eauto.
+          now apply dmut_sub_dcl.
+        + intros x. rewrite dmut_wp_bind_right; auto.
+          rewrite dmut_wp_assume_formula; auto. cbn.
+          rewrite inst_subst, inst_sub_id. intros <-.
+          rewrite dmut_wp_sub. rewrite sub_comp_id_right. revert Hwp.
+          eapply d_dcl; rewrite ?inst_sub_id, ?inst_lift; eauto.
+          now apply dmut_sub_dcl.
+        + intros x.
+          apply dmut_bind_right_dcl.
+          apply dmut_assume_formula_dcl.
+          now apply dmut_sub_dcl.
+    Qed.
 
     Lemma dmut_wp_match_sum {AT A} `{InstLaws AT A} {Γ1 Γ2 Σ1} (x y : 𝑺) (σ τ : Ty) (s : Term Σ1 (ty_sum σ τ))
       (dinl : DynamicMutator Γ1 Γ2 AT (Σ1 ▻ (x :: σ)))  (dinl_dcl : dmut_dcl dinl)
@@ -1547,7 +1617,7 @@ Module Soundness
     Qed.
 
     Lemma bapprox_match_enum {AT A E} `{InstLaws AT A} {Γ1 Γ2 Σ1} (t : Term Σ1 (ty_enum E))
-      (dm : Lit (ty_enum E) -> DynamicMutator Γ1 Γ2 AT Σ1)
+      (dm : Lit (ty_enum E) -> DynamicMutator Γ1 Γ2 AT Σ1) (dm_dcl : forall x, dmut_dcl (dm x))
       (sm : Lit (ty_enum E) -> SCMut Γ1 Γ2 A)
       (ι : SymInstance Σ1) :
       (forall k, bapprox ι (dm k) (sm k)) ->
@@ -1627,7 +1697,7 @@ Module Soundness
       - apply bapprox_produce_chunk.
       - apply bapprox_demonic_binary; apply bapprox_bind_right;
           try apply bapprox_assume_formula; auto using dmut_produce_dcl.
-      - now apply bapprox_match_enum.
+      - apply bapprox_match_enum; auto using dmut_produce_dcl.
       - apply bapprox_match_sum; auto using dmut_produce_dcl.
       - admit.
       - apply bapprox_match_pair; auto using dmut_produce_dcl.
@@ -1639,12 +1709,91 @@ Module Soundness
       - unfold bapprox. intuition.
     Admitted.
 
+    Lemma match_chunk_eqb_spec {Σ} (ce cr : Chunk Σ) (fmls : List Formula Σ) :
+      OptionSpec
+        (fun fmls2 =>
+           forall ι : SymInstance Σ,
+             instpc ι fmls2 ->
+             inst ι ce = inst ι cr /\ instpc ι fmls)
+        True
+        (Soundness.MUT.match_chunk_eqb ce cr fmls).
+    Proof.
+      destruct ce, cr; cbn; try constructor; auto.
+      - destruct (eq_dec p p0); cbn.
+        + destruct e; cbn. admit.
+        + now constructor.
+      - destruct (eq_dec_het r r0); cbn.
+        + dependent elimination e; cbn. admit.
+        + now constructor.
+    Admitted.
+
+    Lemma heap_extractions_map {A B} (f : A -> B) (h : list A) :
+      heap_extractions (List.map f h) = List.map (base.prod_map f (List.map f)) (heap_extractions h).
+    Proof.
+      induction h; cbn.
+      - reflexivity.
+      - f_equal.
+        rewrite IHh.
+        rewrite ?List.map_map.
+        apply List.map_ext.
+        intros [x xs]. reflexivity.
+    Qed.
+
     Lemma bapprox_consume_chunk {Γ Σ} (ι : SymInstance Σ) (c : Chunk Σ) :
       bapprox
         (Γ1 := Γ) (Γ2 := Γ) ι
         (dmut_consume_chunk c)
         (scmut_consume_chunk (inst ι c)).
     Proof.
+      unfold bapprox, dmut_consume_chunk, scmut_consume_chunk.
+      intros * Hι Hpc.
+      unfold dmut_get_heap, scmut_get_heap, scmut_state_heap.
+      rewrite dmut_wp_bind, scmut_wp_bind; auto.
+      rewrite dmut_wp_state.
+      rewrite dmut_wp_bind; auto.
+      rewrite dmut_wp_angelic_list. intros [[Δpc h'] [HIn Hwp]].
+      rewrite subst_sub_id in HIn.
+      cbn - [dmut_wp] in Hwp. rewrite dmut_wp_bind_right in Hwp; auto.
+      rewrite dmut_wp_assert_formulas in Hwp; auto.
+      rewrite ?inst_lift in Hwp. destruct Hwp as [HΔpc Hwp].
+      destruct s1 as [δ1 h1]. cbn [symbolicstate_heap] in HIn. cbn in Hwp.
+      rewrite ?inst_subst, ?inst_lift in Hwp.
+      rewrite scmut_wp_state; cbn - [scmut_wp extract_chunk_eqb].
+      unfold scmut_wp, scmut_angelick_list.
+      rewrite outcome_satisfy_angelick_list.
+      left. exists (inst ι h').
+      split.
+      - apply base.elem_of_list_In in HIn.
+        unfold Soundness.MUT.extract_chunk_eqb, extract_chunk_eqb in *.
+        unfold base.omap in HIn.
+        apply list.elem_of_list_omap in HIn.
+        destruct HIn as [[c' h''] [HIn Heq]].
+        apply List.in_map_iff.
+        destruct (match_chunk_eqb_spec c c' nil); cbn in Heq; try discriminate.
+        inversion Heq. subst h'' a. clear Heq.
+        specialize (H ι). inster H by (subst; auto). destruct H as [H _].
+        exists (inst ι c', inst (T := List Chunk) ι h'). cbn.
+        apply base.elem_of_list_In in HIn.
+        split; auto. apply List.filter_In.
+        split.
+        + unfold lift, inst in HIn. cbn in HIn.
+          rewrite List.map_map in HIn.
+          rewrite heap_extractions_map in HIn.
+          rewrite List.in_map_iff in HIn.
+          destruct HIn as [[c1 h1'] [Heq HIn]].
+          unfold base.prod_map in Heq; cbn in Heq.
+          rewrite <- List.map_map in Heq.
+          change (lift (inst ι1 c1) :: lift (inst ι1 h1') = c' :: h') in Heq.
+          inversion Heq. subst. clear Heq.
+          rewrite ?inst_lift in *.
+          unfold inst at 3. cbn.
+          rewrite heap_extractions_map.
+          rewrite List.in_map_iff.
+          exists (c1, h1'). split; auto.
+        + destruct (MUT.match_chunk_eqb_spec (inst ι c) (inst ι c')); auto.
+      - cbn; now subst.
+      - admit.
+      - admit.
     Admitted.
 
     Lemma bapprox_consume {Γ Σ} (ι : SymInstance Σ) (asn : Assertion Σ) :
@@ -1660,7 +1809,7 @@ Module Soundness
           auto using dmut_consume_dcl.
         apply bapprox_assume_formula.
         apply bapprox_assume_formula.
-      - now apply bapprox_match_enum.
+      - apply bapprox_match_enum; auto using dmut_consume_dcl.
       - apply bapprox_match_sum; auto using dmut_consume_dcl.
       - admit.
       - apply bapprox_match_pair; auto using dmut_consume_dcl.
@@ -1814,11 +1963,18 @@ Module Soundness
         + apply bapprox_bind; auto. admit. admit.
           intros ?. apply bapprox_call.
         + admit.
-      - apply bapprox_bind. admit. admit.
+      - apply bapprox_bind. admit.
+        { apply bapprox_state. destruct s1; cbn; auto. }
         intros δ0. apply bapprox_bind_right.
         apply dmut_bind_left_dcl. apply dmut_exec_dcl.
-        admit. admit. admit.
-      - admit.
+        { apply dmut_state_dcl.
+          destruct s1, s2; intros ? ? -> Heqs Heqζ; inversion Heqs; cbn in *.
+          rewrite ?inst_subst. f_equal. f_equal; congruence. }
+        { apply bapprox_state. destruct s1; cbn; intros.
+          now rewrite inst_subst, inst_lift. }
+        admit.
+      - apply bapprox_bind. admit. admit. intros args.
+        apply bapprox_call.
       - admit.
       - apply bapprox_bind_right; auto. apply dmut_exec_dcl.
       - apply bapprox_bind. admit.
@@ -1914,2089 +2070,23 @@ Module Soundness
 
   End TwoPointOSoundness.
 
-  Module DynMutV1Soundness.
+  Section Leftovers.
 
-    Import DynMutV1.
-
-    Definition DynamicMutatorArrow Γ1 Γ2 A B Σ0 : Type :=
-      forall Σ1, Sub Σ0 Σ1 -> A Σ1 -> DynamicMutator Γ1 Γ2 B Σ1.
-
-    Definition DynamicMutatorArrow' Γ1 Γ2 A B Σ0 : Type :=
-      forall Σ1,
-        Sub Σ0 Σ1 -> A Σ1 -> PathCondition Σ1 ->
-        SymbolicState Γ1 Σ1 -> Outcome (DynamicMutatorError) (DynamicMutatorResult Γ2 B Σ1).
-
-    Definition dmut_bind' {Γ1 Γ2 Γ3 A B Σ0}
-               (ma : DynamicMutator Γ1 Γ2 A Σ0) (f : DynamicMutatorArrow' Γ2 Γ3 A B Σ0) : DynamicMutator Γ1 Γ3 B Σ0 :=
-      fun (Σ1 : LCtx) (ζ01 : Sub Σ0 Σ1) pc1 (s1 : SymbolicState Γ1 Σ1) =>
-        outcome_bind (ma Σ1 ζ01 pc1 s1) (fun r : DynamicMutatorResult Γ2 A Σ1 =>
-        outcome_bind (f (dmutres_context r) (sub_comp ζ01 (dmutres_substitution r)) (dmutres_result_value r) (dmutres_pathcondition r) (dmutres_result_state r))
-                     (fun r2 : DynamicMutatorResult Γ3 B (dmutres_context r) => outcome_pure (cosubst_dmutres (dmutres_substitution r) r2))).
-
-
-    (* A proper preorder on the result of a symbolic execution. *)
-    Definition dmutres_geq {AT A} `{Subst AT, Inst AT A} {Γ Σ} (r1 r2 : DynamicMutatorResult Γ AT Σ) : Prop :=
-      match r1 , r2 with
-      | MkDynMutResult ζ1 pc1 a1 s1, MkDynMutResult ζ2 pc2 a2 s2 =>
-        exists ζ12,
-        pc2 ⊢ subst ζ12 pc1 /\
-        pc2 ⊢ subst ζ12 ζ1 == ζ2 /\
-        pc2 ⊢ subst ζ12 a1 == a2 /\
-        pc2 ⊢ subst ζ12 s1 == s2
-      end.
-
-    Global Instance dmutres_geq_preorder {Γ AT A Σ} `{Subst AT, SubstLaws AT, Inst AT A, InstLaws AT A} : PreOrder (@dmutres_geq AT A _ _ Γ Σ).
+    Lemma subst_lookup {Γ Σ Σ' x σ} (xInΓ : (x ∶ σ)%ctx ∈ Γ) (ζ : Sub Σ Σ') (δ : SymbolicLocalStore Γ Σ) :
+      (subst ζ (δ ‼ x)%exp = (subst ζ δ ‼ x)%exp).
     Proof.
-      split.
-      - intros [ζ1 pc1 a1 s1]. exists (sub_id _).
-        rewrite ?subst_sub_id; easy.
-      - intros [Σ1 ζ1 pc1 a1 s1] [Σ2 ζ2 pc2 a2 s2] [Σ3 ζ3 pc3 a3 s3] (ζ12 & pc21 & ζ12' & a12 & s12) (ζ23 & pc32 & ζ23' & a23 & s23).
-        exists (sub_comp ζ12 ζ23).
-        rewrite ?subst_sub_comp; repeat split.
-        + now rewrite pc32, pc21.
-        + now rewrite <-ζ23', pc32, ζ12'.
-        + now rewrite <-a23, pc32, a12.
-        + now rewrite <-s23, pc32, s12.
+      unfold subst at 2, subst_localstore, SubstEnv.
+      now rewrite env_lookup_map.
     Qed.
 
-    (* A frequent special case. *)
-    Lemma dmutres_geq_syntactic {Γ A V Σ} `{InstLaws A V} :
-      forall r1 r2 : DynamicMutatorResult Γ A Σ,
-        (match r1 , r2 with
-         | MkDynMutResult ζ1 pc1 a1 s1, MkDynMutResult ζ2 pc2 a2 s2 =>
-           exists ζ12,
-           ζ2  = sub_comp ζ1 ζ12 /\
-           pc2 = subst ζ12 pc1 /\
-           a2  = subst ζ12 a1 /\
-           s2  = subst ζ12 s1
-         end
-        ) ->
-        dmutres_geq r1 r2.
+    Lemma subst_symboliceval {Γ τ Σ Σ'} (e : Exp Γ τ) (ζ : Sub Σ Σ') (δ : SymbolicLocalStore Γ Σ) :
+      subst (T := fun Σ => Term Σ _) ζ (symbolic_eval_exp δ e) = symbolic_eval_exp (subst ζ δ) e.
     Proof.
-      intros [Σ1 ζ1 pc1 a1 s1] [Σ2 ζ2 pc2 a2 s2] (ζ12 & ζ12' & pc12 & a12 & s12).
-      exists ζ12; intuition.
-      intros ι ιpc2; intuition.
-    Qed.
-
-
-    Definition dmutres_equiv {AT A} `{Subst AT, Inst AT A} {Γ Σ} (r1 r2 : DynamicMutatorResult Γ AT Σ) : Prop :=
-      dmutres_geq r1 r2 /\ dmutres_geq r2 r1.
-
-    Global Instance dmutres_equiv_equiv {Γ Σ} `{Subst AT, SubstLaws AT, Inst AT A, InstLaws AT A} : Equivalence (@dmutres_equiv _ _ _ _ Γ Σ).
-    Proof.
-      split.
-      - easy.
-      - intros x y [xy yx]; easy.
-      - intros x y z [xy yx] [yz zy]; split; transitivity y; easy.
-    Qed.
-
-    Lemma dmutres_geq_pre_comp {AT A} `{Inst AT A, Subst AT} {Γ Σ}
-          (r1 r2 : DynamicMutatorResult Γ AT Σ) {Σ0} (ζ : Sub Σ0 Σ) :
-        dmutres_geq r1 r2 ->
-        dmutres_geq (cosubst_dmutres ζ r1) (cosubst_dmutres ζ r2).
-    Proof.
-      destruct r1 as [Σ1 ζ1 pc1 a1 s1].
-      destruct r2 as [Σ2 ζ2 pc2 a2 s2].
-      intros [ζ23]. exists ζ23. intuition.
-      unfold sub_comp.
-      now rewrite subst_assoc, H1.
-    Qed.
-
-    Lemma dmutres_try_assume_eq_spec {Γ Σ0 σ} (pc0 : PathCondition Σ0) (t1 t2 : Term Σ0 σ) (s0 : SymbolicState Γ Σ0) :
-      OptionSpec
-        (dmutres_equiv (MkDynMutResult (sub_id _) (cons (formula_eq t1 t2) pc0) tt s0))
-        True
-        (dmutres_try_assume_eq pc0 t1 t2 s0).
-    Proof.
-      destruct t1; cbn; try (constructor; auto; fail).
-      destruct (occurs_check ςInΣ t2) eqn:?; constructor; auto.
-      apply (@occurs_check_sound _ _ (@OccursCheckTerm _) OccursCheckLawsTerm) in Heqo.
-      subst t2.
-      split.
-      - exists (sub_single ςInΣ t).
-        repeat split.
-        + unfold subst at 2, SubstList; cbn.
-          rewrite <-subst_sub_comp, sub_comp_shift_single, subst_sub_id, lookup_sub_single_eq.
-          now rewrite <-entails_cons.
-        + now rewrite subst_sub_id_right.
-      - exists (sub_shift ςInΣ).
-        repeat split; intros ι [eq ιpc]%inst_pathcondition_cons.
-        + now rewrite <-subst_sub_comp, inst_subst, (inst_single_shift ςInΣ t ι eq), inst_sub_id.
-        + refine (inst_single_shift ςInΣ t ι eq).
-        + now rewrite <-subst_sub_comp, inst_subst, (inst_single_shift ςInΣ t ι eq), inst_sub_id.
-    Qed.
-
-    Opaque dmutres_try_assume_eq_spec.
-
-    Lemma dmutres_assume_formula_spec {Γ Σ} (pc : PathCondition Σ) (fml : Formula Σ) (s : SymbolicState Γ Σ) :
-      dmutres_equiv (dmutres_assume_formula pc fml s) (MkDynMutResult (sub_id _) (cons fml pc) tt s).
-    Proof.
-      destruct fml; cbn; try easy.
-      destruct (dmutres_try_assume_eq_spec pc t1 t2 s); try easy. clear H.
-      destruct (dmutres_try_assume_eq_spec pc t2 t1 s); try easy.
-      rewrite <-H.
-      split; cbn; exists (sub_id _);
-        rewrite ?subst_sub_id; intuition;
-          (* do we need a notion of pc-entails-formula and Proper instances for cons-formula-pathcondition? *)
-          intros ι ιpc;
-          rewrite ?inst_pathcondition_cons in *; cbn; intuition.
-    Qed.
-
-    (* Relate two symbolic instances at different points during execution. This
-       essentially encodes a preorder on the total space { Σ & SymInstance Σ },
-       which encodes that ι2 is a future of ι1, i.e. it is derived by compatible
-       for existing variables and values for new universal variables. *)
-    Definition syminstance_rel {Σ1 Σ2} (ζ : Sub Σ1 Σ2) (ι1 : SymInstance Σ1) (ι2 : SymInstance Σ2) : Prop :=
-      inst ι2 ζ = ι1.
-    Hint Unfold syminstance_rel : core.
-
-    Lemma syminstance_rel_refl {Σ} (ι : SymInstance Σ) :
-      syminstance_rel (sub_id Σ) ι ι.
-    Proof. apply inst_sub_id. Qed.
-
-    Lemma syminstance_rel_refl_inv {Σ} (ι1 ι2 : SymInstance Σ) :
-      syminstance_rel (sub_id Σ) ι1 ι2 -> ι2 = ι1.
-    Proof. unfold syminstance_rel. now rewrite inst_sub_id. Qed.
-
-    Lemma syminstance_rel_snoc {Σ1 Σ2 x τ} (ζ : Sub Σ1 Σ2) (ι1 : SymInstance Σ1) ι2 :
-      forall t v,
-        syminstance_rel (env_snoc ζ (x,τ) t) (env_snoc ι1 (x,τ) v) ι2 <->
-        syminstance_rel ζ ι1 ι2 /\ v = inst ι2 t.
-    Proof.
-      unfold syminstance_rel. intros. split.
-      - cbn; intros.
-        now dependent elimination H.
-      - cbn; intros []; subst; now cbn.
-    Qed.
-
-    Lemma syminstance_rel_comp {Σ0 Σ1 Σ2} (ζ1 : Sub Σ0 Σ1) (ζ2 : Sub Σ1 Σ2)
-          (ι0 : SymInstance Σ0) (ι2 : SymInstance Σ2):
-      syminstance_rel (sub_comp ζ1 ζ2) ι0 ι2 <->
-      syminstance_rel ζ1 ι0 (inst ι2 ζ2).
-    Proof. unfold syminstance_rel. now rewrite <- inst_subst. Qed.
-
-    Lemma syminstance_rel_trans {Σ0 Σ1 Σ2} {ζ1 : Sub Σ0 Σ1} {ζ2 : Sub Σ1 Σ2}
-          {ι0 : SymInstance Σ0} {ι1 : SymInstance Σ1} {ι2 : SymInstance Σ2} :
-      syminstance_rel ζ1 ι0 ι1 -> syminstance_rel ζ2 ι1 ι2 ->
-      syminstance_rel (sub_comp ζ1 ζ2) ι0 ι2.
-    Proof. intros. apply syminstance_rel_comp. congruence. Qed.
-
-    Lemma syminstance_rel_wk1 {Σ : NCtx 𝑺 Ty} {x τ} (ι : SymInstance Σ) (v : Lit τ) :
-      syminstance_rel sub_wk1 ι (ι ► ((x, τ) ↦ v)).
-    Proof. apply inst_sub_wk1. Qed.
-
-    Lemma syminstance_rel_up {Σ1 Σ2 x τ} (ζ : Sub Σ1 Σ2) (ι1 : SymInstance Σ1) ι2 :
-      forall v,
-        syminstance_rel (sub_up1 ζ) (env_snoc ι1 (x,τ) v) (env_snoc ι2 (x,τ) v) <->
-        syminstance_rel ζ ι1 ι2.
-    Proof.
-      unfold syminstance_rel. intros v.
-      change (inst (ι2 ► (x :: τ ↦ v)) (sub_comp ζ sub_wk1) ► (x :: τ ↦ v) =
-              ι1 ► (x :: τ ↦ v) <-> inst ι2 ζ = ι1).
-      unfold sub_comp. rewrite inst_subst, inst_sub_wk1.
-      split; intros H.
-      - now dependent elimination H.
-      - now f_equal.
-    Qed.
-
-    Section StateProp.
-
-      Definition StateProperty Γ A Σ :=
-        forall Σ1, Sub Σ Σ1 -> PathCondition Σ1 -> A Σ1 -> SymbolicState Γ Σ1 -> Prop.
-
-      Definition stateprop_downwards_closed {Γ Σ AT A} `{Inst AT A} `{Subst AT} (p : StateProperty Γ AT Σ) : Prop :=
-        forall Σ1 (ζ1 : Sub Σ Σ1) pc1 a1 s1 Σ2 (ζ2 : Sub Σ Σ2) pc2 a2 s2,
-          dmutres_geq (MkDynMutResult ζ1 pc1 a1 s1) (MkDynMutResult ζ2 pc2 a2 s2) ->
-          p Σ1 ζ1 pc1 a1 s1 -> p Σ2 ζ2 pc2 a2 s2.
-
-      (* The property always holds vacuously on inconsistent paths. *)
-      Definition stateprop_vacuous {Γ AT Σ} (p : StateProperty Γ AT Σ) : Prop :=
-        forall Σ1 (ζ1 : Sub Σ Σ1) pc a1 s1, inconsistent pc -> p Σ1 ζ1 pc a1 s1.
-
-      Definition stateprop_impl {Γ A Σ} (P Q : StateProperty Γ A Σ) : Prop :=
-        forall Σ1 (ζ : Sub Σ Σ1) (pc : PathCondition Σ1) (a : A Σ1) (s : SymbolicState Γ Σ1),
-          P Σ1 ζ pc a s -> Q Σ1 ζ pc a s.
-
-      Definition stateprop_specialize {Γ A Σ1 Σ2} (ζ : Sub Σ1 Σ2) (p: StateProperty Γ A Σ1) :
-        StateProperty Γ A Σ2 := fun Σ3 ζ3 => p Σ3 (sub_comp ζ ζ3).
-
-      Definition stateprop_lift {Γ AT A Σ} {instA : Inst AT A} (ι : SymInstance Σ) (POST : A -> SCState Γ -> Prop) :
-        StateProperty Γ AT Σ :=
-        fun Σ1 ζ1 pc1 v1 s1 =>
-          forall ι1,
-            syminstance_rel ζ1 ι ι1 ->
-            (inst ι1 pc1 : Prop) ->
-            POST (inst ι1 v1) (inst ι1 s1).
-
-      Lemma stateprop_lift_dcl {Γ AT A Σ1} `{Inst AT A} `{InstLaws AT A} (ι1 : SymInstance Σ1) (POST : A -> SCState Γ -> Prop) :
-        stateprop_downwards_closed (stateprop_lift ι1 POST).
-      Proof.
-        unfold stateprop_downwards_closed, stateprop_lift.
-        intros Σ2 ζ2 pc2 a2 s2 Σ3 ζ3 pc3 a3 s3.
-        intros [ζ23 (pc23 & ζ23' & a23 & s23)] Hpost ι3 rel13 Hpc3.
-        specialize (Hpost (inst ι3 ζ23)).
-        unfold syminstance_rel in Hpost, rel13.
-        rewrite <-?inst_subst, (ζ23' ι3 Hpc3), (a23 ι3 Hpc3), (s23 ι3 Hpc3) in Hpost.
-        intuition.
-      Qed.
-
-      Lemma stateprop_lift_vac {Γ AT A Σ1} `{Inst AT A} (ι1 : SymInstance Σ1) (POST : A -> SCState Γ -> Prop) :
-        stateprop_vacuous (stateprop_lift ι1 POST).
-      Proof. unfold stateprop_vacuous, stateprop_lift. intuition. Qed.
-
-    End StateProp.
-
-    Section ResultProp.
-
-      Definition ResultProperty Γ A Σ :=
-        DynamicMutatorResult Γ A Σ -> Prop.
-
-      Definition resultprop_specialize {Γ A Σ1 Σ2} (ζ : Sub Σ1 Σ2) :
-        ResultProperty Γ A Σ1 -> ResultProperty Γ A Σ2 :=
-        fun p r => p (cosubst_dmutres ζ r).
-
-      Definition resultprop_downwards_closed {Γ AT Σ A} `{Inst AT A, Subst AT} (p : ResultProperty Γ AT Σ) : Prop :=
-        forall (r1 r2 : DynamicMutatorResult Γ AT Σ),
-          dmutres_geq r1 r2 -> p r1 -> p r2.
-
-      Definition resultprop_vacuous {Γ AT Σ A} `{Inst AT A} (p : ResultProperty Γ AT Σ) : Prop :=
-        forall r, inconsistent (dmutres_pathcondition r) -> p r.
-
-      Lemma resultprop_specialize_vac {Γ A AV Σ1 Σ2} `{Inst A AV} (ζ : Sub Σ1 Σ2)
-            (P : ResultProperty Γ A Σ1) (P_vac : resultprop_vacuous P) :
-        resultprop_vacuous (resultprop_specialize ζ P).
-      Proof.
-        intros [Σ3 ζ23 pc3 a3 s3]; unfold resultprop_specialize; cbn.
-        intros HYP. apply P_vac; auto.
-      Qed.
-
-      Lemma resultprop_specialize_dcl {Γ A AV Σ1 Σ2} `{InstLaws A AV} (ζ : Sub Σ1 Σ2)
-            (POST : ResultProperty Γ A Σ1) (POST_dcl : resultprop_downwards_closed POST) :
-        resultprop_downwards_closed (resultprop_specialize ζ POST).
-      Proof.
-        unfold resultprop_downwards_closed, resultprop_specialize.
-        eauto using POST_dcl, dmutres_geq_pre_comp.
-      Qed.
-
-      Lemma resultprop_specialize_id {Γ A Σ} (P : ResultProperty Γ A Σ) :
-        forall r, resultprop_specialize (sub_id _) P r <-> P r.
-      Proof.
-        intros [Σ' ζ pc a s]; unfold resultprop_specialize; cbn.
-        now rewrite sub_comp_id_left.
-      Qed.
-
-      Lemma resultprop_specialize_comp {Γ A Σ1 Σ2 Σ3} (ζ12 : Sub Σ1 Σ2) (ζ23 : Sub Σ2 Σ3) (P : ResultProperty Γ A Σ1) :
-        forall r,
-          resultprop_specialize (sub_comp ζ12 ζ23) P r <->
-          resultprop_specialize ζ23 (resultprop_specialize ζ12 P) r.
-      Proof.
-        intros [Σ' ζ pc a s]; unfold resultprop_specialize; cbn.
-        now rewrite sub_comp_assoc.
-      Qed.
-
-      Definition resultprop_lift {Γ AT A Σ1} {instA : Inst AT A} (ι1 : SymInstance Σ1) (POST : A -> SCState Γ -> Prop) :
-        ResultProperty Γ AT Σ1 :=
-        fun dres =>
-          match dres with
-          | MkDynMutResult ζ2 pc2 a2 s2 =>
-            stateprop_lift ι1 POST ζ2 pc2 a2 s2
-          end.
-
-      Definition resultprop_lift_dcl {Γ AT A Σ1} `{InstLaws AT A} (ι1 : SymInstance Σ1) (POST : A -> SCState Γ -> Prop) :
-        resultprop_downwards_closed (resultprop_lift ι1 POST).
-      Proof.
-        unfold resultprop_downwards_closed, resultprop_lift.
-        intros [Σ3 ζ3 pc3 a3 s3] [Σ4 ζ4 pc4 a4 s4].
-        apply stateprop_lift_dcl.
-      Qed.
-
-      Definition resultprop_lift_vac {Γ AT A Σ1} `{InstLaws AT A} (ι1 : SymInstance Σ1) (POST : A -> SCState Γ -> Prop) :
-        resultprop_vacuous (resultprop_lift ι1 POST).
-      Proof.
-        unfold resultprop_vacuous, resultprop_lift, stateprop_lift.
-        intros [Σ2 ζ2 pc2 a2 s2] Hpc2; cbn in *. intuition.
-      Qed.
-
-
-      Global Instance resultprop_lift_proper {Γ AT A Σ} `{InstLaws AT A} {ι : SymInstance Σ} {POST : A -> SCState Γ -> Prop} :
-        Proper (dmutres_geq ==> impl) (resultprop_lift ι POST) := resultprop_lift_dcl _ _.
-
-      Global Instance resultprop_lift_proper_equiv {Γ AT A Σ} `{InstLaws AT A} {ι : SymInstance Σ} {POST : A -> SCState Γ -> Prop} :
-        Proper (dmutres_equiv ==> impl) (resultprop_lift ι POST).
-      Proof.
-        intros r1 r2 (r12 & r21).
-        now eapply resultprop_lift_proper.
-      Qed.
-
-
-    End ResultProp.
-
-    Section Vacuous.
-
-      Definition outcome_vac `{Inst AT A} {Γ Σ} (pc : PathCondition Σ) (o : Outcome (DynamicMutatorError) (DynamicMutatorResult Γ AT Σ)) : Prop :=
-        forall (P : ResultProperty Γ AT Σ) (P_vac : resultprop_vacuous P),
-          inconsistent pc -> outcome_satisfy o contradiction P.
-      Local Hint Unfold outcome_satisfy : core.
-      Local Hint Unfold outcome_vac : core.
-
-      Definition dmut_vac `{Inst AT A} {Γ1 Γ2 Σ0} (d : DynamicMutator Γ1 Γ2 AT Σ0) : Prop :=
-        forall Σ1 (ζ01 : Sub Σ0 Σ1) pc1 s1, outcome_vac pc1 (d Σ1 ζ01 pc1 s1).
-      Local Hint Unfold dmut_vac : core.
-
-      (* TODO: It would be great to reformulate this to use the above. *)
-      Definition dmut_arrow_vac `{Inst AT A, Inst BT B} {Γ1 Γ2 Σ0}
-        (f : DynamicMutatorArrow Γ1 Γ2 AT BT Σ0) : Prop :=
-        forall Σ1 (ζ01 : Sub Σ0 Σ1) pc1 (a1 : AT Σ1) s1,
-          outcome_vac pc1 (f Σ1 ζ01 a1 Σ1 (sub_id _) pc1 s1).
-      Local Hint Unfold dmut_arrow_vac : core.
-
-      Definition dmut_arrow_vac' `{Inst AT A, Inst BT B} {Γ1 Γ2 Σ0}
-        (f : DynamicMutatorArrow' Γ1 Γ2 AT BT Σ0) : Prop :=
-        forall Σ1 (ζ01 : Sub Σ0 Σ1) pc1 (a1 : AT Σ1) s1,
-          outcome_vac pc1 (f Σ1 ζ01 a1 pc1 s1).
-      Local Hint Unfold dmut_arrow_vac' : core.
-
-      Lemma dmut_pure_vac `{Subst AT, Inst AT A} {Γ Σ} (a : AT Σ) :
-        dmut_vac (dmut_pure (Γ := Γ) a).
-      Proof. unfold dmut_pure; auto. Qed.
-      Local Hint Resolve dmut_pure_vac : core.
-
-      Lemma dmut_block_vac `{Inst AT A} {Γ1 Γ2 Σ} :
-        dmut_vac (@dmut_block Γ1 Γ2 AT Σ).
-      Proof. unfold dmut_block; auto. Qed.
-      Local Hint Resolve dmut_block_vac : core.
-
-      Lemma dmut_contradiction_vac `{Inst AT A} {D Γ1 Γ2 Σ} func msg data :
-        dmut_vac (@dmut_contradiction Γ1 Γ2 AT Σ D func msg data).
-      Proof.
-        unfold dmut_contradiction, dmut_vac, outcome_vac; cbn; intros.
-        constructor; auto. constructor; auto.
-      Qed.
-      Local Hint Resolve dmut_contradiction_vac : core.
-
-      Lemma dmut_fail_vac `{Inst AT A} {D Γ1 Γ2 Σ} func msg data :
-        dmut_vac (@dmut_fail Γ1 Γ2 AT Σ D func msg data).
-      Proof. unfold dmut_fail, dmut_vac, outcome_vac, contradiction; cbn; auto. Qed.
-      Local Hint Resolve dmut_fail_vac : core.
-
-      Lemma dmut_bind_vac' `{Inst AT A, Inst BT B} {Γ1 Γ2 Γ3 Σ0}
-        (d : DynamicMutator Γ1 Γ2 AT Σ0) (vac_d : dmut_vac d)
-        (f : DynamicMutatorArrow' Γ2 Γ3 AT BT Σ0) (vac_f : dmut_arrow_vac' f) :
-        dmut_vac (dmut_bind' d f).
-      Proof.
-        unfold dmut_bind', dmut_vac, outcome_vac; cbn.
-        intros Σ1 ζ1 pc1 s1 P Pvac incpc1.
-        rewrite outcome_satisfy_bind.
-        eapply vac_d; auto.
-        intros [Σ2 ζ2 pc2 a2 s2] ιpc2; cbn.
-        rewrite outcome_satisfy_bind.
-        eapply vac_f; auto.
-        intros [Σ3 ζ3 pc3 a3 s3] ιpc3; cbn.
-        now eapply Pvac.
-      Qed.
-      Local Hint Resolve dmut_bind_vac' : core.
-
-      Lemma dmut_bind_vac `{Inst AT A, Inst BT B} {Γ1 Γ2 Γ3 Σ0}
-        (d : DynamicMutator Γ1 Γ2 AT Σ0) (vac_d : dmut_vac d)
-        (f : DynamicMutatorArrow Γ2 Γ3 AT BT Σ0) (vac_f : dmut_arrow_vac f) :
-        dmut_vac (dmut_bind d f).
-      Proof.
-        unfold dmut_bind, dmut_vac, outcome_vac; cbn.
-        intros Σ1 ζ1 pc1 s1 P Pvac incpc1.
-        rewrite outcome_satisfy_bind.
-        eapply vac_d; auto.
-        intros [Σ2 ζ2 pc2 a2 s2] ιpc2; cbn.
-        rewrite outcome_satisfy_bind.
-        eapply vac_f; auto.
-        intros [Σ3 ζ3 pc3 a3 s3] ιpc3; cbn.
-        now eapply Pvac.
-      Qed.
-      Local Hint Resolve dmut_bind_vac : core.
-
-      Lemma dmut_sub_vac `{Inst AT A} {Γ1 Γ2 Σ0} (d : DynamicMutator Γ1 Γ2 AT Σ0) (vac_d : dmut_vac d) :
-        forall (Σ1 : LCtx) (ζ1 : Sub Σ0 Σ1), dmut_vac (dmut_sub ζ1 d).
-      Proof. unfold dmut_sub; auto. Qed.
-      Local Hint Resolve dmut_sub_vac : core.
-
-      Lemma dmut_bind_right_vac `{Inst AT A, Inst BT B} {Γ1 Γ2 Γ3 Σ0}
-        (d1 : DynamicMutator Γ1 Γ2 AT Σ0) (d2 : DynamicMutator Γ2 Γ3 BT Σ0) (vac_d1 : dmut_vac d1) (vac_d2 : dmut_vac d2) :
-        dmut_vac (dmut_bind_right d1 d2).
-      Proof. unfold dmut_bind_right; eauto. Qed.
-      Local Hint Resolve dmut_bind_right_vac : core.
-
-      Local Hint Extern 5 (outcome_vac _ (dmut_bind_right _ _ _ _ _)) =>
-        apply dmut_bind_right_vac : core.
-      Local Hint Extern 5 (outcome_vac _ (dmut_bind _ _ _ _ _)) =>
-        apply dmut_bind_vac; unfold dmut_arrow_vac; intros; destruct_conjs : core.
-      Local Hint Extern 5 (outcome_vac _ (dmut_pure _ _ _ _)) =>
-        apply dmut_pure_vac : core.
-
-      Lemma dmut_fmap_vac `{Subst AT, Subst BT, Inst AT A, Inst BT B} {Γ1 Γ2 Σ0}
-            (da : DynamicMutator Γ1 Γ2 AT Σ0) (da_vac : dmut_vac da)
-            (f : forall Σ1, Sub Σ0 Σ1 -> AT Σ1 -> BT Σ1) :
-        dmut_vac (dmut_fmap da f).
-      Proof. unfold dmut_fmap; auto. Qed.
-      Local Hint Resolve dmut_fmap_vac : core.
-
-      Lemma dmut_fmap2_vac `{Subst AT, Subst BT, Subst CT, Inst AT A, Inst BT B, Inst CT C} {Γ1 Γ2 Γ3 Σ0}
-            (da : DynamicMutator Γ1 Γ2 AT Σ0) (da_vac : dmut_vac da)
-            (db : DynamicMutator Γ2 Γ3 BT Σ0) (db_vac : dmut_vac db)
-            (f : forall Σ1, Sub Σ0 Σ1 -> AT Σ1 -> BT Σ1 -> CT Σ1) :
-        dmut_vac (dmut_fmap2 da db f).
-      Proof. unfold dmut_fmap2; auto. Qed.
-      Local Hint Resolve dmut_fmap2_vac : core.
-
-      Lemma dmut_pair_vac `{Subst AT, Subst BT, Inst AT A, Inst BT B} {Γ1 Γ2 Γ3 Σ0}
-            (da : DynamicMutator Γ1 Γ2 AT Σ0) (da_vac : dmut_vac da)
-            (db : DynamicMutator Γ2 Γ3 BT Σ0) (db_vac : dmut_vac db) :
-        dmut_vac (dmut_pair da db).
-      Proof. unfold dmut_pair; eauto. Qed.
-      Local Hint Resolve dmut_pair_vac : core.
-      Local Hint Unfold outcome_satisfy : core.
-
-      Lemma dmut_demonic_binary_vac `{Inst AT A} {Γ1 Γ2 Σ0}
-        (d1 d2 : DynamicMutator Γ1 Γ2 AT Σ0) (vac_d1 : dmut_vac d1) (vac_d2 : dmut_vac d2) :
-        dmut_vac (dmut_demonic_binary d1 d2).
-      Proof.
-        unfold dmut_demonic_binary.
-        unfold dmut_vac in *.
-        unfold outcome_vac in *.
-        now cbn; eauto.
-      Qed.
-
-      Local Hint Resolve dmut_demonic_binary_vac : core.
-
-      Local Hint Extern 5 (outcome_vac _ (dmut_demonic_binary _ _ _ _ _)) =>
-        apply dmut_demonic_binary_vac : core.
-
-      Lemma dmut_angelic_binary_vac `{Inst AT A} {Γ1 Γ2 Σ0}
-        (d1 d2 : DynamicMutator Γ1 Γ2 AT Σ0) (vac_d1 : dmut_vac d1) (vac_d2 : dmut_vac d2) :
-        dmut_vac (dmut_angelic_binary d1 d2).
-      Proof.
-        unfold dmut_angelic_binary.
-        unfold dmut_vac in *.
-        unfold outcome_vac in *.
-        now cbn; eauto.
-      Qed.
-      Local Hint Resolve dmut_angelic_binary_vac : core.
-
-      Lemma dmut_angelic_list_vac {AT A} `{Subst AT, Inst AT A} {Γ1 Γ2 Σ}
-            {D} {func : string} {msg : string} {data:D}
-            (l : list (DynamicMutator Γ1 Γ2 AT Σ)) :
-        List.Forall dmut_vac l ->
-        dmut_vac (dmut_angelic_list func msg data l).
-      Proof.
-        induction 1 as [|r rs vacr vacrs]; cbn; eauto.
-        generalize rs at 1.
-        intros rs'; destruct rs'; auto.
-      Qed.
-      Local Hint Resolve dmut_angelic_list_vac : core.
-
-      Lemma dmut_demonic_vac {Γ1 Γ2 I AT Σ} `{Inst AT A} {ms : I -> DynamicMutator Γ1 Γ2 AT Σ} :
-        (forall i, dmut_vac (ms i)) ->
-        dmut_vac (dmut_demonic ms).
-      Proof.
-        unfold dmut_demonic, dmut_vac, outcome_vac in *; cbn; eauto.
-      Qed.
-      Local Hint Resolve dmut_demonic_vac : core.
-
-      Lemma dmut_demonic_list_vac {AT A} {F : Type} `{Subst AT, Inst AT A} {Γ1 Γ2 Σ} (l : list (DynamicMutator Γ1 Γ2 AT Σ)) :
-        List.Forall dmut_vac l ->
-        dmut_vac (dmut_demonic_list l).
-      Proof.
-        induction 1 as [|r rs vacr vacrs]; cbn; eauto.
-        generalize rs at 1.
-        intros rs'; destruct rs'; auto.
-      Qed.
-      Local Hint Resolve dmut_demonic_list_vac : core.
-
-      Lemma dmut_demonic_finite_vac {AT A} {F : Type} `{Subst AT, Inst AT A, finite.Finite F} {Γ Σ} (k : F -> DynamicMutator Γ Γ AT Σ) :
-        (forall v, dmut_vac (k v)) ->
-        dmut_vac (dmut_demonic_finite F k).
-      Proof.
-        intros kvac.
-        unfold dmut_demonic_finite.
-        enough (List.Forall dmut_vac (List.map k (finite.enum F))) by eauto.
-        eapply List.Forall_forall.
-        intros x [f [eq fInF]]%List.in_map_iff.
-        subst x.
-        now eapply kvac.
-      Qed.
-      Local Hint Resolve dmut_demonic_finite_vac : core.
-
-      Lemma dmut_angelic_finite_vac {AT A} {F : Type} `{Subst AT, Inst AT A, finite.Finite F} {Γ Σ} (k : F -> DynamicMutator Γ Γ AT Σ) :
-        (forall v, dmut_vac (k v)) ->
-        dmut_vac (dmut_angelic_finite F k).
-      Proof.
-        intros kvac.
-        unfold dmut_angelic_finite.
-        enough (List.Forall dmut_vac (List.map k (finite.enum F))) by eauto.
-        eapply List.Forall_forall.
-        intros x [f [eq fInF]]%List.in_map_iff.
-        subst x.
-        now eapply kvac.
-      Qed.
-      Local Hint Resolve dmut_angelic_finite_vac : core.
-
-      Lemma dmut_state_vac {AT A} `{Inst AT A} {Γ1 Γ2 Σ} (f : forall Σ' : LCtx, Sub Σ Σ' -> SymbolicState Γ1 Σ' -> AT Σ' * SymbolicState Γ2 Σ') :
-        dmut_vac (dmut_state f).
-      Proof.
-        unfold dmut_vac, dmut_state, outcome_vac; intros.
-        destruct (f Σ1 ζ01 s1); cbn. now apply P_vac.
-      Qed.
-      Local Hint Resolve dmut_state_vac : core.
-
-      Lemma inconsistent_cons {Σ} {pc : PathCondition Σ} {f : Formula Σ} :
-        inconsistent pc -> inconsistent (f :: pc)%list.
-      Proof.
-        intros ipc ι; cbn; unfold instpc, inst_pathcondition; cbn.
-        rewrite fold_right_1_10_prop.
-        intros [Hf Hl].
-        exact (ipc _ Hl).
-      Qed.
-
-      Lemma dmutres_assume_formula_inconsistent {Γ Σ Σ1} {f : Formula Σ} {ζ1 : Sub Σ Σ1}
-            {pc1 : PathCondition Σ1} {s1 : SymbolicState Γ Σ1} :
-        inconsistent pc1 ->
-        inconsistent (dmutres_pathcondition (dmutres_assume_formula pc1 (subst ζ1 f) s1)).
-      Proof.
-        intros ipc1 ι Hpc2.
-        destruct (dmutres_assume_formula_spec pc1 (subst ζ1 f) s1) as [_ geq2].
-        revert ι Hpc2 geq2.
-        generalize (dmutres_assume_formula pc1 (subst ζ1 f) s1).
-        intros [Σ2 ζ2 pc2 a2 s2] ι Hpc2 [ζ (pc21 & _)].
-        cbn in *.
-        eapply (ipc1 (inst ι ζ)).
-        specialize (pc21 ι Hpc2).
-        unfold inst, instantiate_pathcondition, inst_pathcondition in pc21.
-        cbn in pc21.
-        rewrite fold_right_1_10_prop in pc21.
-        destruct pc21 as (Hf & Hpc1).
-        change (instpc ι (subst ζ pc1)) in Hpc1.
-        now rewrite inst_subst in Hpc1.
-      Qed.
-
-      Lemma dmut_assume_formula_vac {Γ Σ} (f : Formula Σ) :
-        dmut_vac (@dmut_assume_formula Γ Σ f).
-      Proof.
-        unfold dmut_assume_formula.
-        intros Σ1 ζ1 pc1 s1.
-        destruct (try_solve_formula (subst ζ1 f)).
-        - destruct b; auto.
-        - intros P Pvac inc1.
-          unfold outcome_satisfy; cbn.
-          now eapply Pvac, dmutres_assume_formula_inconsistent.
-      Qed.
-      Local Hint Resolve dmut_assume_formula_vac : core.
-
-      Lemma dmut_assume_formulas_vac {Γ Σ} (pc : PathCondition Σ) :
-        dmut_vac (@dmut_assume_formulas Γ Σ pc).
-      Proof.
-        unfold dmut_assume_formulas.
-        induction pc; cbn; eauto.
-      Qed.
-      Local Hint Resolve dmut_assume_formulas_vac : core.
-
-      Lemma dmut_modify_vac {Γ Γ' Σ} (f : forall Σ', Sub Σ Σ' -> SymbolicState Γ Σ' -> SymbolicState Γ' Σ') :
-        dmut_vac (dmut_modify f).
-      Proof.
-        unfold dmut_modify; eauto.
-      Qed.
-      Local Hint Resolve dmut_modify_vac : core.
-
-      Lemma dmut_produce_chunk_vac {Γ Σ} (c : Chunk Σ) :
-        dmut_vac (@dmut_produce_chunk Γ Σ c).
-      Proof.
-        unfold dmut_produce_chunk; eauto.
-      Qed.
-      Local Hint Resolve dmut_produce_chunk_vac : core.
-
-      Lemma dmut_fresh_vac {AT A} `{Inst AT A} {Γ Σ σ x} (d : DynamicMutator Γ Γ AT (Σ ▻ (x :: σ))) (d_vac : dmut_vac d) :
-        dmut_vac (dmut_fresh x σ d).
-      Proof.
-        unfold dmut_fresh, dmut_vac.
-        intros Σ1 ζ01 pc1 s1 P Pvac ipc1.
-        rewrite outcome_satisfy_map.
-        eapply d_vac.
-        - intros [Σ2 ζ2 pc2 a2 s2] incr.
-          now eapply Pvac.
-        - intros ι Hpc1.
-          unfold wk1 in Hpc1.
-          rewrite inst_subst in Hpc1.
-          now eapply (ipc1 (inst ι sub_wk1)).
-      Qed.
-
-      Local Hint Resolve dmut_fresh_vac : core.
-
-      Lemma dmut_freshtermvar_vac {Γ Σ σ x} :
-        dmut_vac (@dmut_freshtermvar Γ Σ σ x).
-      Proof. unfold dmut_freshtermvar; auto. Qed.
-      Local Hint Resolve dmut_freshtermvar_vac : core.
-
-      Lemma dmut_freshen_recordpat'_vac {Γ Σ σs Δ} (p : RecordPat σs Δ) :
-        dmut_vac (@dmut_freshen_recordpat' 𝑺 id σs Δ p Γ Σ).
-      Proof. induction p; cbn; eauto. Qed.
-      Local Hint Resolve dmut_freshen_recordpat'_vac : core.
-
-      Lemma dmut_freshen_recordpat_vac {Γ Σ R Δ} (p : RecordPat (𝑹𝑭_Ty R) Δ) :
-        dmut_vac (@dmut_freshen_recordpat 𝑺 id R Δ p Γ Σ).
-      Proof. unfold dmut_freshen_recordpat; eauto. Qed.
-      Local Hint Resolve dmut_freshen_recordpat_vac : core.
-
-      Lemma dmut_produce_vac {Γ Σ} (asn : Assertion Σ) :
-        dmut_vac (@dmut_produce Γ Σ asn).
-      Proof.
-        induction asn; cbn [dmut_produce]; unfold dmut_assume_term; eauto.
-        - apply dmut_bind_vac; auto.
-          unfold dmut_arrow_vac; intros.
-          destruct (term_get_sum a1) as [[]|]; eauto 10.
-        - destruct (term_get_pair s) as [[]|]; eauto 10.
-        (* - apply dmut_bind_vac; auto. *)
-        (*   unfold dmut_arrow_vac; intros. *)
-        (*   destruct (term_get_record a1); eauto. *)
-        (* - destruct (term_get_union s) as [[]|]; eauto. *)
-      Admitted.
-      Local Hint Resolve dmut_produce_vac : core.
-
-      Lemma dmut_assert_formula_vac {Γ Σ} (f : Formula Σ) :
-        dmut_vac (@dmut_assert_formula Γ Σ f).
-      Proof.
-        unfold dmut_assert_formula.
-        intros Σ1 ζ1 pc1 s1.
-        destruct (try_solve_formula (subst ζ1 f)).
-        - destruct b; auto.
-        - intros P Pvac inc1.
-          unfold outcome_satisfy; cbn.
-          split.
-          + constructor. clear s1.
-            eapply Forall_forall.
-            intros E ιpc1.
-            exfalso; eapply inc1; eauto.
-          + now eapply Pvac, dmutres_assume_formula_inconsistent.
-      Qed.
-      Local Hint Resolve dmut_assert_formula_vac : core.
-
-      Lemma dmut_modify_heap_vac {Γ Σ}
-            (f : forall Σ', Sub Σ Σ' -> SymbolicHeap Σ' -> SymbolicHeap Σ') :
-        dmut_vac (@dmut_modify_heap Γ Σ f).
-      Proof.
-        unfold dmut_modify_heap; eauto.
-      Qed.
-      Local Hint Resolve dmut_modify_heap_vac : core.
-
-      Lemma dmut_put_heap_vac {Γ Σ} (h : SymbolicHeap Σ) :
-        dmut_vac (@dmut_put_heap Γ Σ h).
-      Proof.
-        unfold dmut_put_heap; eauto.
-      Qed.
-      Local Hint Resolve dmut_put_heap_vac : core.
-
-      Lemma dmut_get_heap_vac {Γ Σ} :
-        dmut_vac (@dmut_get_heap Γ Σ).
-      Proof.
-        unfold dmut_get_heap; eauto.
-      Qed.
-      Local Hint Resolve dmut_get_heap_vac : core.
-
-      Lemma dmut_consume_chunk_vac {Γ Σ} (c : Chunk Σ) :
-        dmut_vac (@dmut_consume_chunk Γ Σ c).
-      Proof.
-        unfold dmut_consume_chunk.
-        eapply dmut_bind_vac; eauto.
-        intros Σ2 ζ2 pc2 a2 s2.
-        eapply dmut_angelic_list_vac.
-        eapply List.Forall_forall.
-        intros d [[pc3 h2] (eq & r)]%List.in_map_iff.
-        subst d; eauto.
-      Qed.
-      Local Hint Resolve dmut_consume_chunk_vac : core.
-
-      Lemma dmut_angelic_vac {Γ1 Γ2 I AT A Σ} `{Inst AT A}
-            {ms : I -> DynamicMutator Γ1 Γ2 AT Σ} :
-        (exists i, dmut_vac (ms i)) ->
-        dmut_vac (dmut_angelic ms).
-      Proof.
-        unfold dmut_angelic.
-        intros [i msvac] Σ1 ζ1 pc1 s1 P Pvac Hpc1.
-        cbn. exists i. now eapply msvac.
-      Qed.
-
-      Lemma dmut_consume_vac {Γ Σ} (asn : Assertion Σ) :
-        dmut_vac (@dmut_consume Γ Σ asn).
-      Proof.
-        induction asn; cbn [dmut_consume];
-          unfold dmut_assert_term, dmut_assume_term; eauto 10.
-        - destruct (term_get_sum s) as [[s'|s']|s']; eauto.
-          eapply dmut_angelic_binary_vac.
-          + eapply dmut_angelic_vac.
-            admit.
-          + eapply dmut_angelic_vac.
-            admit.
-        - destruct (term_get_pair s) as [[t1 t2]|].
-          eauto.
-          eapply dmut_angelic_vac.
-          admit.
-        - destruct (term_get_record s).
-          eauto.
-          eapply dmut_angelic_vac.
-          admit.
-      Admitted.
-      Local Hint Resolve dmut_consume_vac : core.
-
-      Lemma dmut_call_vac {Γ Δ τ Σ} (c : SepContract Δ τ) (ts : NamedEnv (Term Σ) Δ) :
-        dmut_vac (@dmut_call Γ Δ τ Σ c ts).
-      Proof. Admitted.
-      Local Hint Resolve dmut_call_vac : core.
-
-      Lemma dmut_eval_exp_vac {Γ σ} {e : Exp Γ σ} {Σ} :
-        dmut_vac (dmut_eval_exp (Σ := Σ) e).
-      Proof.
-        unfold dmut_eval_exp, dmut_gets_local, dmut_gets; eauto.
-      Qed.
-      Local Hint Resolve dmut_eval_exp_vac : core.
-
-      Lemma dmut_eval_exps_vac {Γ Σ} {σs : PCtx} (es : NamedEnv (Exp Γ) σs) :
-        dmut_vac (dmut_eval_exps (Σ := Σ) es).
-      Proof.
-        unfold dmut_eval_exps, dmut_gets_local, dmut_gets; eauto.
-      Qed.
-      Local Hint Resolve dmut_eval_exps_vac : core.
-
-      Ltac auto_vac :=
-        repeat (
-          match goal with
-          | |- dmut_vac (dmut_bind _ _) => eapply dmut_bind_vac
-          | |- dmut_arrow_vac ?f => intros Σ3 ζ3 pc3 a3 s3
-          | |- outcome_vac ?pc (dmut_bind_right _ _ _ _ _) =>
-            eapply dmut_bind_right_vac
-          | |- outcome_vac ?pc (dmut_assume_formula _ _ _ _) =>
-            eapply dmut_assume_formula_vac
-          | |- dmut_vac (dmut_bind_right _ _) => eapply dmut_bind_right_vac
-          | |- dmut_vac (dmut_demonic_binary _ _) =>
-            eapply dmut_demonic_binary_vac
-          | |- outcome_vac ?pc (dmut_fresh _ _ _ _ _ _ _) =>
-            eapply dmut_fresh_vac
-          | |- dmut_vac (dmut_fresh _ _ _) =>
-            eapply dmut_fresh_vac
-          | |- outcome_vac ?pc (dmut_demonic _ _ _ _) =>
-            eapply dmut_demonic_vac
-          | |- outcome_vac ?pc (dmut_demonic_binary _ _ _ _ _) =>
-            eapply dmut_demonic_binary_vac
-          | |- outcome_vac ?pc (dmut_call _ _ _ _ _) => eapply dmut_call_vac
-          | |- outcome_vac _ (match ?e with _ => _ end _ _ _ _) => destruct e
-          end; eauto).
-
-      Lemma dmut_exec_vac {Γ Σ τ} (s : Stm Γ τ) :
-        dmut_vac (@dmut_exec Γ τ Σ s).
-      Proof.
-        revert Σ.
-        induction s; intros Σ; cbn [dmut_exec];
-          unfold dmut_assume_exp, dmut_assume_term, dmut_eval_exps, dmut_eval_exp, dmut_put_local, dmut_pop_local, dmut_pushs_local, dmut_pops_local, dmut_push_local, dmut_modify_local, dmut_get_local, dmut_gets_local, dmut_gets, dmut_state_local, dmut_bind_left; eauto; auto_vac.
-        - admit.
-        - admit.
-      Admitted.
-      Local Hint Resolve dmut_exec_vac : core.
-
-      Lemma dmut_leakcheck_vac {Γ Σ} :
-        dmut_vac (@dmut_leakcheck Γ Σ).
-      Proof.
-        unfold dmut_leakcheck.
-        eapply dmut_bind_vac; eauto.
-        intros Σ1 ζ1 pc1 [|a hp]; eauto.
-      Qed.
-      Local Hint Resolve dmut_leakcheck_vac : core.
-
-      Lemma dmut_contract_vac {Γ τ} (c : SepContract Γ τ) (s : Stm Γ τ)  :
-        dmut_vac (@dmut_contract Γ τ c s).
-      Proof.
-        destruct c; cbn; eauto 10.
-        apply dmut_bind_right_vac; eauto 10.
-        apply dmut_bind_vac; eauto 10.
-        unfold dmut_arrow_vac; intros.
-        eapply dmut_sub_vac; eauto 10.
-      Qed.
-
-    End Vacuous.
-
-    Definition resultprop_specialize_pc {Γ A Σ1 Σ2} (ζ : Sub Σ1 Σ2) (pc2 : PathCondition Σ2) :
-      ResultProperty Γ A Σ1 -> ResultProperty Γ A Σ2 :=
-      fun p r => dmutres_pathcondition r ⊢ subst (dmutres_substitution r) pc2 /\ p (cosubst_dmutres ζ r).
-
-    Lemma resultprop_specialize_pc_vac {Γ A AV Σ1 Σ2} `{InstLaws A AV}
-          (ζ12 : Sub Σ1 Σ2) (pc2 : PathCondition Σ2)
-          (POST : ResultProperty Γ A Σ1) (POST_vac : resultprop_vacuous POST) :
-      resultprop_vacuous (resultprop_specialize_pc ζ12 pc2 POST).
-    Proof.
-      intros [Σ3 ζ23 pc3 a3 s3] incpc; cbn in *.
-      unfold resultprop_specialize_pc; cbn.
-      split.
-      - intros ι Hpc3. exfalso. eapply (incpc _ Hpc3).
-      - eapply POST_vac; now cbn.
-    Qed.
-
-    Lemma resultprop_specialize_pc_dcl {Γ A AV Σ1 Σ2} `{InstLaws A AV}
-          (ζ12 : Sub Σ1 Σ2) (pc2 : PathCondition Σ2)
-          (POST : ResultProperty Γ A Σ1) (POST_dcl : resultprop_downwards_closed POST) :
-      resultprop_downwards_closed (resultprop_specialize_pc ζ12 pc2 POST).
-    Proof.
-      unfold resultprop_downwards_closed, resultprop_specialize_pc.
-      intros r3 r4 r34 [Hpc23 Hpost].
-      split.
-      - destruct r3 as [Σ3 ζ23 pc3 a3 s3].
-        destruct r4 as [Σ4 ζ24 pc4 a4 s4].
-        destruct r34 as [ζ34 ?].
-        cbn in *. destruct_conjs.
-        rewrite <- H4, <- subst_assoc.
-        transitivity (subst ζ34 pc3); auto.
-        now rewrite Hpc23.
-      - refine (POST_dcl _ _ _ Hpost).
-        now eapply dmutres_geq_pre_comp.
-    Qed.
-
-    Definition dmut_dcl {Γ1 Γ2 AT Σ0 A} `{Inst AT A, Subst AT} (d : DynamicMutator Γ1 Γ2 AT Σ0) : Prop :=
-      forall Σ1 Σ2 (ζ01 : Sub Σ0 Σ1) pc1 (s1 : SymbolicState Γ1 Σ1) (ζ12 : Sub Σ1 Σ2) pc2 s2 ζ02,
-        pc2 ⊢ subst ζ12 pc1 ->
-        pc2 ⊢ subst ζ12 s1 == s2 ->
-        pc2 ⊢ subst ζ12 ζ01 == ζ02 ->
-        forall (P : ResultProperty Γ2 AT Σ1) (P_dcl : resultprop_downwards_closed P) (P_vac : resultprop_vacuous P)
-               (Q : ResultProperty Γ2 AT Σ2) (PQ : forall r, resultprop_specialize_pc ζ12 pc2 P r -> Q r),
-          outcome_satisfy (d Σ1 ζ01 pc1 s1) contradiction P ->
-          outcome_satisfy (d Σ2 ζ02 pc2 s2) contradiction Q.
-
-    Definition dmut_arrow_dcl {Γ1 Γ2 AT A BT B Σ0} `{Inst AT A, Subst AT, Inst BT B, Subst BT}
-               (f : DynamicMutatorArrow Γ1 Γ2 AT BT Σ0) : Prop :=
-      forall Σ1 Σ2 Σ3 Σ4 (ζ01 : Sub Σ0 Σ1) (ζ12 : Sub Σ1 Σ2) (ζ03 : Sub Σ0 Σ3) (ζ34 : Sub Σ3 Σ4) (ζ24 : Sub Σ2 Σ4) (pc2 : PathCondition Σ2) (pc4 : PathCondition Σ4) (a1 : AT Σ1) (a3 : AT Σ3) (s2 : SymbolicState Γ1 Σ2) (s4 : SymbolicState Γ1 Σ4),
-        pc4 ⊢ subst ζ24 pc2 ->
-        pc4 ⊢ subst (subst ζ24 ζ12) ζ01 == subst ζ34 ζ03 ->
-        pc4 ⊢ subst (subst ζ24 ζ12) a1 == subst ζ34 a3 ->
-        pc4 ⊢ subst ζ24 s2 == s4 ->
-        forall (P : ResultProperty Γ2 BT Σ2) (P_dcl : resultprop_downwards_closed P) (P_vac : resultprop_vacuous P)
-          (Q : ResultProperty Γ2 BT Σ4) (PQ : forall r, resultprop_specialize_pc ζ24 pc4 P r -> Q r),
-          outcome_satisfy (f Σ1 ζ01 a1 Σ2 ζ12 pc2 s2) contradiction P ->
-          outcome_satisfy (f Σ3 ζ03 a3 Σ4 ζ34 pc4 s4) contradiction Q.
-
-    Lemma dmut_bind_dcl {AT A BT B} `{InstLaws BT B} `{InstLaws AT A}
-          {Γ1 Γ2 Γ3 Σ0} (d : DynamicMutator Γ1 Γ2 AT Σ0) (d_dcl : dmut_dcl d)
-          (f : DynamicMutatorArrow Γ2 Γ3 AT BT Σ0)
-          (f_dcl : dmut_arrow_dcl f)
-          (f_vac : dmut_arrow_vac f) :
-      dmut_dcl (dmut_bind d f).
-    Proof.
-      unfold dmut_bind.
-      intros Σ1 Σ2 ζ01 pc1 s1 ζ12 pc2 s2 ζ02 Hpc12 Hs12 Hζ12 P P_dcl P_vac Q PQ.
-      rewrite ?outcome_satisfy_bind; cbn.
-      eapply d_dcl; eauto.
-      - clear - f_dcl P P_dcl P_vac H2 H6.
-        unfold resultprop_downwards_closed.
-        intros [Σ2 ζ12 pc2 a2 s2] [Σ3 ζ13 pc3 a3 s3] [ζ23 (Hpc23 & Hζ23 & Ha23 & Hs23)]; cbn in *.
-        rewrite ?outcome_satisfy_bind; cbn.
-        eapply f_dcl; eauto.
-        + rewrite subst_sub_id_right, subst_sub_id.
-          repeat unfold sub_comp.
-          now rewrite subst_assoc, Hζ23.
-        + now rewrite subst_sub_id, subst_sub_id_right.
-        + (* rewrite inside bind? *)
-          unfold resultprop_downwards_closed.
-          intros [] [] Hgeq; cbn - [dmutres_geq].
-          apply P_dcl.
-          exact (dmutres_geq_pre_comp _ _ ζ12 Hgeq).
-        + unfold resultprop_vacuous.
-          intros [] Hpc; cbn in *. now apply P_vac.
-        + intros [Σ4 ζ34 pc4 b4 s4]; unfold resultprop_specialize_pc; cbn.
-          intros [Hpc34 HP]; revert HP. apply P_dcl.
-          exists (sub_id _).
-          rewrite ?subst_sub_id.
-          unfold sub_comp.
-          repeat split; try easy.
-          now rewrite Hpc34, <-subst_assoc, Hζ23.
-      - intros [Σ3 ζ23 pc3 a3 s3]; cbn.
-        rewrite outcome_satisfy_bind; cbn.
-        apply f_vac.
-        intros [Σ4 ζ34 pc4 a4 s4]; cbn.
-        intros.
-        now apply P_vac.
-      - intros [Σ3 ζ23 pc3 a3 s3]; unfold resultprop_specialize_pc; cbn.
-        rewrite ?outcome_satisfy_bind; cbn.
-        intros [Hpc23 Hpost]; revert Hpost.
-        eapply f_dcl; rewrite ?subst_sub_id; try easy.
-        + clear - Hζ12 Hpc23.
-          unfold sub_comp.
-          now rewrite <-subst_assoc, Hpc23, Hζ12.
-        + unfold resultprop_downwards_closed.
-          intros [] [] Hgeq; cbn - [dmutres_geq].
-          apply P_dcl.
-          exact (dmutres_geq_pre_comp _ _ (sub_comp ζ12 ζ23) Hgeq).
-        + unfold resultprop_vacuous.
-          intros [] Hpc; cbn in *. now apply P_vac.
-        + intros [Σ4 ζ34 pc4 b4 s4]; unfold resultprop_specialize_pc; cbn.
-          intros [Hpc34 Hpost].
-          eapply PQ. split; cbn; unfold sub_comp.
-          * now rewrite <-subst_assoc, <-Hpc23.
-          * rewrite sub_comp_id_left in Hpost.
-            unfold sub_comp in Hpost.
-            now rewrite subst_assoc in Hpost.
-    Qed.
-
-    (* These should be kept abstract in the rest of the proof. If you need some
-       property, add a lemma above. *)
-    Local Opaque dmutres_try_assume_eq.
-    Local Opaque dmutres_assume_formula.
-
-    Section DownwardsClosure.
-
-      Definition dmut_dcl' {Γ1 Γ2 AT Σ0 A} `{Inst AT A, Subst AT} (d : DynamicMutator Γ1 Γ2 AT Σ0) : Prop :=
-        forall Σ1 Σ2 (ζ01 : Sub Σ0 Σ1) pc1 (s1 : SymbolicState Γ1 Σ1) (ζ12 : Sub Σ1 Σ2) pc2 s2 ζ02,
-          pc2 ⊢ subst ζ12 pc1 ->
-          pc2 ⊢ subst ζ12 s1 == s2 ->
-          pc2 ⊢ subst ζ12 ζ01 == ζ02 ->
-          forall (P : ResultProperty Γ2 AT Σ1) (P_dcl : resultprop_downwards_closed P) (P_vac : resultprop_vacuous P),
-            outcome_satisfy (d Σ1 ζ01 pc1 s1) contradiction P ->
-            outcome_satisfy (d Σ2 ζ02 pc2 s2) contradiction (resultprop_specialize_pc ζ12 pc2 P).
-
-      Lemma dmut_dcl_dcl' {Γ1 Γ2 AT Σ0 A} `{Inst AT A, Subst AT}
-            (d : DynamicMutator Γ1 Γ2 AT Σ0) :
-        dmut_dcl d <-> dmut_dcl' d.
-      Proof.
-        split.
-        - unfold dmut_dcl, dmut_dcl'.
-          intros d_dcl * Hpc12 Hs12 Hζ12 P P_dcl P_vac.
-          eapply d_dcl; eauto.
-        - unfold dmut_dcl, dmut_dcl'.
-          intros d_dcl * Hpc12 Hs12 Hζ12 P P_dcl P_vac Q PQ.
-          intros HP. eapply d_dcl in HP; eauto. revert HP.
-          apply outcome_satisfy_monotonic. intros r. apply PQ.
-      Qed.
-
-      Lemma dmut_pure_dcl {Γ AT Σ A} {subA: Subst AT} {sublAT: SubstLaws AT}
-            {instA : Inst AT A} {instlA : InstLaws AT A} (a : AT Σ) :
-        dmut_dcl (dmut_pure (Γ := Γ) a).
-      Proof.
-        unfold dmut_dcl, dmut_pure.
-        intros * Hpc12 Hs12 Hζ12 P P_dcl P_vac Q PQ HP.
-        cbn in *.
-        eapply PQ.
-        unfold resultprop_specialize_pc.
-        cbn; rewrite subst_sub_id; intuition.
-        revert HP. eapply P_dcl.
-        exists ζ12; unfold sub_comp;
-          rewrite ?subst_sub_id, ?subst_sub_id_right, subst_assoc, Hζ12; easy.
-      Qed.
-
-      Lemma dmut_fail_dcl `{Inst AT A, Subst AT} {D Γ1 Γ2 Σ} func msg data :
-        dmut_dcl (@dmut_fail Γ1 Γ2 AT Σ D func msg data).
-      Proof.
-        apply dmut_dcl_dcl'.
-        unfold dmut_dcl', dmut_fail, contradiction, inconsistent, not; cbn.
-        intros. unfold entails in H1. apply (H4 (inst ι ζ12)).
-        rewrite <- inst_subst. intuition.
-      Qed.
-
-      Lemma dmut_sub_dcl {Γ1 Γ2 AT A Σ0} `{Inst AT A, Subst AT} (d : DynamicMutator Γ1 Γ2 AT Σ0) (d_dcl : dmut_dcl d) :
-        forall (Σ1 : LCtx) (ζ1 : Sub Σ0 Σ1), dmut_dcl (dmut_sub ζ1 d).
-      Proof.
-        unfold dmut_dcl, dmut_sub.
-        intros * Hpc12 Hs12 Hζ12 P P_dcl Q PQ.
-        eapply d_dcl; eauto. unfold sub_comp.
-        now rewrite subst_assoc, Hζ12.
-      Qed.
-
-      Lemma dmut_bind_right_dcl `{InstLaws AT A, InstLaws BT B} {Γ1 Γ2 Γ3 Σ0}
-        (d1 : DynamicMutator Γ1 Γ2 AT Σ0) (d2 : DynamicMutator Γ2 Γ3 BT Σ0)
-        (d1_dcl : dmut_dcl d1) (d2_dcl : dmut_dcl d2) (d2_vac : dmut_vac d2) :
-        dmut_dcl (dmut_bind_right d1 d2).
-      Proof.
-        unfold dmut_bind_right.
-        apply dmut_bind_dcl; auto.
-        - unfold dmut_arrow_dcl.
-          intros until Q. intros PQ.
-          unfold dmut_sub; cbn.
-          eapply d2_dcl; eauto.
-          unfold sub_comp; now rewrite subst_assoc.
-        - unfold dmut_arrow_vac.
-          intros.
-          now apply dmut_sub_vac.
-      Qed.
-
-      Lemma dmut_demonic_binary_dcl {Γ1 Γ2 AT A Σ0} `{Inst AT A, Subst AT} (d1 d2 : DynamicMutator Γ1 Γ2 AT Σ0) (d_wf1 : dmut_dcl d1) (d_wf2 : dmut_dcl d2) :
-        dmut_dcl (dmut_demonic_binary d1 d2).
-      Proof.
-        unfold dmut_dcl, dmut_demonic_binary; cbn.
-        intros * Hpc12 Hs12 Hζ12 P P_dcl P_vac Q PQ [H1 H2].
-        split.
-        - revert PQ H1. apply d_wf1; auto.
-        - revert PQ H2. apply d_wf2; auto.
-      Qed.
-
-      Lemma dmut_angelic_binary_dcl {Γ1 Γ2 AT A Σ0} `{Inst AT A, Subst AT} (d1 d2 : DynamicMutator Γ1 Γ2 AT Σ0) (d1_dcl : dmut_dcl d1) (d2_dcl : dmut_dcl d2) :
-        dmut_dcl (dmut_angelic_binary d1 d2).
-      Proof.
-        unfold dmut_dcl, dmut_angelic_binary. cbn.
-        intros * Hpc12 Hs12 Hζ12 P P_dcl P_vac Q PQ [H1|H1].
-        - left. revert PQ H1. apply d1_dcl; auto.
-        - right. revert PQ H1. apply d2_dcl; auto.
-      Qed.
-
-      (* Redo these once the new definition of dmut_dcl is ready. *)
-
-      (* Lemma dmut_state_dcl {AT A} `{Inst AT A} {Γ1 Γ2 Σ} *)
-      (*       (f : forall Σ' : LCtx, Sub Σ Σ' -> SymbolicState Γ1 Σ' -> AT Σ' * SymbolicState Γ2 Σ') *)
-      (*       (f_dcl : True) : *)
-      (*   dmut_dcl (dmut_state f). *)
-      (* Proof. *)
-      (*   (* unfold dmut_dcl, dmut_state; intros until Q. intros PQ. *) *)
-      (*   (* destruct (f Σ1 ζ01 s1) eqn:?, (f Σ2 ζ02 s2) eqn:?; cbn. *) *)
-      (*   (* intros Hp. apply PQ. split; cbn. apply geqpc_refl. *) *)
-      (*   (* revert Hp. rewrite sub_comp_id_right. *) *)
-      (*   (* apply P_dcl. exists ζ12. *) *)
-      (* Admitted. *)
-      (* Local Hint Resolve dmut_state_dcl : core. *)
-
-      Lemma dmut_assume_formula_dcl {Γ Σ} (f : Formula Σ) :
-        dmut_dcl (@dmut_assume_formula Γ Σ f).
-      Proof.
-        apply dmut_dcl_dcl'. unfold dmut_assume_formula, dmut_dcl'.
-        intros * Hpc12 Hs12 Hζ12 P P_dcl P_vac H.
-        remember (dmutres_assume_formula pc2 (subst ζ02 f) s2) as r.
-        destruct (try_solve_formula_spec (subst ζ01 f));
-        destruct (try_solve_formula_spec (subst ζ02 f)); cbn in *.
-        - clear r Heqr. destruct a, a0; cbn in *; auto.
-          + split; cbn. rewrite subst_sub_id; easy.
-            revert H. apply P_dcl.
-            exists ζ12. rewrite sub_comp_id_right, subst_sub_id_right; easy.
-          + apply resultprop_specialize_pc_vac; cbn; auto.
-            intros ι Hpc2. specialize (Hζ12 ι Hpc2).
-            specialize (H0 (inst ι ζ12)). specialize (H1 ι).
-            rewrite inst_subst in H0. rewrite inst_subst in H1.
-            rewrite inst_subst in Hζ12.
-            rewrite Hζ12 in H0. clear - H0 H1. intuition.
-        - clear H1. destruct a; cbn in *; auto.
-          + subst r. pose proof (dmutres_assume_formula_spec pc2 (subst ζ02 f) s2) as Hgeq.
-            destruct (dmutres_assume_formula pc2 (subst ζ02 f) s2) as [Σ3 ζ23 pc3 [] s3]; cbn in *.
-            destruct Hgeq as [_ [ζ (Hpc23 & Hζ23 & _ & Hs23)]].
-            split; cbn.
-            * intros ι2 Hpc3. specialize (Hpc23 ι2 Hpc3).
-              rewrite subst_sub_id_right in Hζ23.
-              specialize (Hζ23 ι2 Hpc3).
-              change _ with (instpc ι2 (subst ζ (subst ζ02 f) :: subst ζ pc2)%list) in Hpc23.
-              rewrite inst_pathcondition_cons in Hpc23. destruct Hpc23 as [Hf Hpc23].
-              now rewrite inst_subst, Hζ23, <-inst_subst in Hpc23.
-            * revert H. apply P_dcl. cbn. exists (sub_comp ζ12 ζ23).
-              rewrite subst_sub_id_right in Hζ23.
-              rewrite subst_sub_id_right.
-              change _ with (pc3 ⊢ (subst ζ (subst ζ02 f) :: subst ζ pc2)%list) in Hpc23.
-              rewrite <- entails_cons in Hpc23.
-              destruct Hpc23 as [Hpc23 Hf].
-              repeat split; try easy; rewrite subst_sub_comp.
-              now rewrite <-Hζ23, <-Hpc12.
-              rewrite <-Hζ23.
-              transitivity (subst ζ s2); try easy.
-              now rewrite Hpc23, Hs12.
-          + subst r. pose proof (dmutres_assume_formula_spec pc2 (subst ζ02 f) s2) as Hgeq.
-            destruct (dmutres_assume_formula pc2 (subst ζ02 f) s2) as [Σ3 ζ23 pc3 [] s3]; cbn in *.
-            destruct Hgeq as [_ [ζ' (Hpc23 & Hζ23 & _ & Hs23)]].
-            split; cbn in *.
-            * rewrite <-entails_cons in Hpc23. destruct Hpc23 as [Hpc23 Hf].
-              rewrite subst_sub_id_right in Hζ23.
-              now rewrite <-Hζ23.
-            * clear - P_vac H0 Hζ12 Hpc23 Hpc12.
-              eapply P_vac; cbn.
-              rewrite Hpc23.
-              intros ι Hpc3.
-              rewrite inst_pathcondition_cons in Hpc3.
-              destruct Hpc3 as [Hf Hpc2].
-              rewrite inst_subst in Hpc2.
-              rewrite subst_assoc in Hf.
-              specialize (H0 (inst ι (sub_comp ζ12 ζ'))).
-              enough (is_true false) by inversion H.
-              eapply H0; clear H0.
-              rewrite <-inst_subst, subst_sub_comp, inst_subst, subst_assoc.
-              rewrite <-subst_assoc,inst_subst, inst_subst in Hf.
-              now rewrite <-(Hζ12 (inst ι ζ') Hpc2), <-inst_subst in Hf.
-        - clear H0 r Heqr. destruct a; cbn; auto. split; cbn.
-          now rewrite subst_sub_id.
-          rewrite sub_comp_id_right.
-          refine (P_dcl _ _ _ H).
-          transitivity ({| dmutres_context := Σ1;
-                           dmutres_substitution := sub_id Σ1;
-                           dmutres_pathcondition := (subst ζ01 f :: pc1)%list;
-                           dmutres_result_value := tt;
-                           dmutres_result_state := s1
-                        |}).
-          exact (proj1 (dmutres_assume_formula_spec pc1 (subst ζ01 f) s1)).
-          exists ζ12. rewrite subst_sub_id_right, Hs12; repeat split; try easy.
-          change _ with (pc2 ⊢ subst ζ12 (subst ζ01 f) :: subst ζ12 pc1)%list.
-          rewrite <-entails_cons, subst_assoc, Hζ12; intuition.
-          intros ι Hpc2.
-          now eapply H1.
-        - clear H0 H1. subst r.
-          pose proof (dmutres_assume_formula_spec pc2 (subst ζ02 f) s2) as Hgeq.
-          destruct (dmutres_assume_formula pc2 (subst ζ02 f) s2) as [Σ3 ζ23 pc3 [] s3]; cbn in *.
-          destruct Hgeq as [_ [ζ' (Hpc23 & Hζ23 & _ & Hs23)]].
-          rewrite subst_sub_id_right in Hζ23.
-          change _ with (pc3 ⊢ subst ζ' (subst ζ02 f) :: subst ζ' pc2)%list in Hpc23.
-          rewrite <-entails_cons in Hpc23.
-          destruct Hpc23 as [Hpc23 Hf].
-          rewrite Hζ23 in Hs23, Hpc23.
-          split; cbn; auto.
-          * refine (P_dcl _ _ _ H).
-            refine (transitivity (proj1 (dmutres_assume_formula_spec pc1 (subst ζ01 f) s1)) _).
-            exists (sub_comp ζ12 ζ23).
-            rewrite ?subst_sub_comp, subst_sub_id_right, <-Hs23.
-            repeat split; try easy.
-            change _ with (pc3 ⊢ subst ζ23 (subst ζ12 (subst ζ01 f)) :: subst ζ23 (subst ζ12 pc1))%list.
-            rewrite <-entails_cons; split.
-            now rewrite Hpc23, Hpc12.
-            rewrite (subst_assoc _ _ ζ12), <-Hζ23.
-            apply (proper_subst_entails_eq (ζ := ζ23)) in Hζ12.
-            rewrite <-Hpc23,<-Hζ23 in Hζ12.
-            now rewrite subst_assoc, Hζ12, <-subst_assoc.
-            transitivity (subst ζ23 s2); try easy.
-            now rewrite Hpc23, Hs12.
-      Qed.
-
-      (* Lemma dmut_produce_chunk_dcl {Γ Σ} (c : Chunk Σ) : *)
-      (*   dmut_dcl (@dmut_produce_chunk Γ Σ c). *)
-      (* Proof. Admitted. *)
-
-      (* Lemma dmut_fresh_dcl {AT A} `{Inst AT A} {Γ Σ σ x} (d : DynamicMutator Γ Γ AT (Σ ▻ (x :: σ))) (d_dcl : dmut_dcl d) : *)
-      (*   dmut_dcl (dmut_fresh (x :: σ) d). *)
-      (* Proof. Admitted. *)
-
-      (* Lemma dmut_freshtermvar_dcl {Γ Σ σ x} : *)
-      (*   dmut_dcl (@dmut_freshtermvar Γ Σ σ x). *)
-      (* Proof. *)
-      (*   apply dmut_dcl_dcl'. unfold dmut_dcl', dmut_freshtermvar; cbn - [dmut_fresh]. *)
-      (*   intros * Hpc12 Hs12 Hζ12 P P_dcl P_vac. *)
-      (*   eapply dmut_fresh_dcl; eauto. *)
-      (*   apply dmut_pure_dcl. *)
-      (* Qed. *)
-
-      (* Lemma dmut_produce_dcl {Γ Σ} (asn : Assertion Σ) : *)
-      (*   dmut_dcl (@dmut_produce Γ Σ asn). *)
-      (* Proof. *)
-      (*   induction asn; cbn [dmut_produce]; unfold dmut_assume_term. *)
-      (*   - apply dmut_assume_formula_dcl. *)
-      (*   - apply dmut_produce_chunk_dcl. *)
-      (*   - apply dmut_demonic_binary_dcl. *)
-      (*     apply dmut_bind_right_dcl; *)
-      (*       auto using dmut_assume_formula_dcl, dmut_produce_vac. *)
-      (*     apply dmut_bind_right_dcl; *)
-      (*       auto using dmut_assume_formula_dcl, dmut_produce_vac. *)
-      (*   - admit. *)
-      (*   - admit. *)
-      (*   - apply dmut_fail_dcl. *)
-      (*   - admit. *)
-      (*   - apply dmut_fail_dcl. *)
-      (*   - admit. *)
-      (*   - admit. *)
-      (*   - apply dmut_bind_right_dcl; auto using dmut_produce_vac. *)
-      (*   - now apply dmut_fresh_dcl. *)
-      (* Admitted. *)
-
-      (* Lemma dmut_consume_dcl {Γ Σ} (asn : Assertion Σ) : *)
-      (*   dmut_dcl (@dmut_consume Γ Σ asn). *)
-      (* Proof. Admitted. *)
-
-      (* Lemma dmut_exec_dcl {Γ Σ τ} (s : Stm Γ τ) : *)
-      (*   dmut_dcl (@dmut_exec Γ τ Σ s). *)
-      (* Proof. Admitted. *)
-
-      Lemma dmut_contract_dcl {Γ τ} (c : SepContract Γ τ) (s : Stm Γ τ) :
-        dmut_dcl (@dmut_contract Γ τ c s).
-      Proof. Admitted.
-
-    End DownwardsClosure.
-
-    Ltac auto_dcl :=
-      try
-        match goal with
-        | |- dmut_dcl _ => admit
-        | |- dmut_arrow_dcl _ => admit
-        end.
-
-    Definition scmut_wp {Γ1 Γ2 A}
-      (m : SCMut Γ1 Γ2 A)
-      (POST : A -> SCState Γ2 -> Prop)
-      (s1 : SCState Γ1) : Prop :=
-      outcome_satisfy (m s1) (fun _ => False) (fun r => POST (scmutres_value r) (scmutres_state r)).
-
-    Lemma scmut_wp_bind {Γ1 Γ2 Γ3 A B} (ma : SCMut Γ1 Γ2 A) (f : A -> SCMut Γ2 Γ3 B)
-          (POST : B -> SCState Γ3 -> Prop) :
-      forall s1 : SCState Γ1,
-        scmut_wp (scmut_bind ma f) POST s1 <->
-        scmut_wp ma (fun a => scmut_wp (f a) POST) s1.
-    Proof.
-      unfold SCMut, scmut_bind, scmut_wp in *; cbn; intros.
-      now rewrite outcome_satisfy_bind.
-    Qed.
-
-    Definition dmut_wp {Γ1 Γ2 Σ0 Σ1 A}
-      (m : DynamicMutator Γ1 Γ2 A Σ0)
-      (POST : StateProperty Γ2 A Σ0)
-      (ζ1 : Sub Σ0 Σ1)
-      (pc1 : PathCondition Σ1)
-      (s1 : SymbolicState Γ1 Σ1) : Prop :=
-        outcome_satisfy
-          (m Σ1 ζ1 pc1 s1)
-          contradiction
-          (fun '(MkDynMutResult ζ2 pc2 a2 s2) =>
-             POST _ (sub_comp ζ1 ζ2) pc2 a2 s2).
-
-    Lemma dmut_wp_monotonic {Γ1 Γ2 Σ0 A} (m : DynamicMutator Γ1 Γ2 A Σ0)
-          (P Q : StateProperty Γ2 A Σ0) (HYP : stateprop_impl P Q) :
-      forall {Σ1} (ζ : Sub Σ0 Σ1) (pc : PathCondition Σ1) (s : SymbolicState Γ1 Σ1),
-        dmut_wp m P ζ pc s -> dmut_wp m Q ζ pc s.
-    Proof.
-      unfold dmut_wp; cbn; intros Σ1 ζ1 pc1 s1.
-      apply outcome_satisfy_monotonic.
-      intros [Σ2 ζ2 pc2 a2 s2]; cbn.
-      intuition.
-    Qed.
-
-    Lemma dmut_wp_angelic {A B Γ1 Γ2 Σ0} (m : B Σ0 -> DynamicMutator Γ1 Γ2 A Σ0)
-          {Σ1} (ζ01 : Sub Σ0 Σ1) (POST : StateProperty Γ2 A Σ1) :
-      forall {Σ2} (ζ12 : Sub Σ1 Σ2) pc2 s2,
-        dmut_wp (dmut_sub ζ01 (dmut_angelic m)) POST ζ12 pc2 s2 <->
-        exists b, dmut_wp (dmut_sub ζ01 (m b)) POST ζ12 pc2 s2.
-    Proof. reflexivity. Qed.
-
-    Definition dmut_wp_sub_id {Γ1 Γ2 Σ0 A} (m : DynamicMutator Γ1 Γ2 A Σ0) (P : StateProperty Γ2 A Σ0) :
-      forall Σ1 (ζ01 : Sub Σ0 Σ1) (pc1 : PathCondition Σ1) (s1 : SymbolicState Γ1 Σ1),
-      dmut_wp (dmut_sub (sub_id _) m) P ζ01 pc1 s1 <-> dmut_wp m P ζ01 pc1 s1.
-    Proof.
-      unfold dmut_wp, dmut_sub. intros.
-      now rewrite ?sub_comp_id_left.
-    Qed.
-
-    Definition APPROX Γ1 Γ2 AT A {instA : Inst AT A} : Type :=
-      forall Σ (ι : SymInstance Σ),
-        DynamicMutator Γ1 Γ2 AT Σ -> SCMut Γ1 Γ2 A -> Prop.
-    Arguments APPROX _ _ _ _ {_}.
-
-    Definition box {Γ1 Γ2 AT A} {instA : Inst AT A} (R : APPROX Γ1 Γ2 AT A) : APPROX Γ1 Γ2 AT A :=
-      fun Σ ι dm sm =>
-        forall Σ1 (ζ1 : Sub Σ Σ1) (ι1 : SymInstance Σ1),
-          syminstance_rel ζ1 ι ι1 ->
-          R Σ1 ι1 (dmut_sub ζ1 dm) sm.
-
-    Lemma box_proj {Γ1 Γ2 AT A} {instA : Inst AT A} (R : APPROX Γ1 Γ2 AT A) :
-      forall Σ (ι : SymInstance Σ) dm sm,
-        box R ι dm sm -> R _ ι dm sm.
-    Proof.
-      intros ? ? ? ? b.
-      unfold box in b.
-      inster b by apply syminstance_rel_refl.
-      unfold dmut_sub in b.
-      (* apply b. *)
-    Abort.
-
-    Definition box_box {Γ1 Γ2 AT A} {instA : Inst AT A} (R : APPROX Γ1 Γ2 AT A) :
-      forall Σ (ι : SymInstance Σ) dm sm,
-        box R ι dm sm -> box (box R) ι dm sm.
-    Proof.
-      intros ? ? ? ?. unfold box. intros bb Σ1 ζ1 ι1 ? Σ2 ζ2 ι2 ?.
-      specialize (bb Σ2 (sub_comp ζ1 ζ2) ι2).
-      inster bb by eapply syminstance_rel_trans; eauto.
-      (* apply bb. *)
-    Abort.
-
-    Definition approximates {Γ1 Γ2 AT A} {instA : Inst AT A} : APPROX Γ1 Γ2 AT A :=
-      fun Σ ι dm sm =>
-        forall Σ1 (ζ : Sub Σ Σ1) pc (s__sym : SymbolicState Γ1 Σ1) ι1 (POST : A -> SCState Γ2 -> Prop)
-               (Heqι : ι = inst ι1 ζ)
-               (Hpc : inst ι1 pc : Prop)
-               (Hwp : dmut_wp dm (stateprop_lift ι POST) ζ pc s__sym),
-          scmut_wp sm POST (inst ι1 s__sym).
-
-    Lemma approximates_proj {Γ1 Γ2 AT A} {instA : Inst AT A} {Σ} (ι : SymInstance Σ)
-      (dm : DynamicMutator Γ1 Γ2 AT Σ) (sm : SCMut Γ1 Γ2 A) :
-      box approximates ι dm sm -> approximates ι dm sm.
-    Proof.
-      (* unfold approximates, box. intros Happrox * Hdwp Hpc. *)
-      (* inster Happrox by apply syminstance_rel_refl. *)
-      (* specialize (Happrox pc). apply Happrox; auto. *)
-      (* unfold dmut_wp, dmut_sub. intros Σ1 ζ1. *)
-      (* rewrite sub_comp_id_left. apply Hdwp. *)
-    Admitted.
-
-    Lemma approximates_box_box {Γ1 Γ2 AT A} {instA : Inst AT A} {Σ} (ι : SymInstance Σ)
-      (dm : DynamicMutator Γ1 Γ2 AT Σ) (sm : SCMut Γ1 Γ2 A) :
-      box approximates ι dm sm -> box (box approximates) ι dm sm.
-    Proof.
-      (* unfold approximates, box, dmut_wp, dmut_sub. intros. *)
-      (* inster H by eapply syminstance_rel_trans; eauto. *)
-      (* specialize (H pc). apply H; auto. *)
-      (* intros. now rewrite sub_comp_assoc. *)
-    Admitted.
-
-    Lemma approximates_sub {Γ Σ Σ1} (ζ1 : Sub Σ Σ1) (ι : SymInstance Σ) (ι1 : SymInstance Σ1)
-      (relι1 : syminstance_rel ζ1 ι ι1) (d : DynamicMutator Γ Γ Unit Σ) (s : SCMut Γ Γ unit) :
-      box approximates ι d s -> box approximates ι1 (dmut_sub ζ1 d) s.
-    Proof. intros H. eapply approximates_box_box; eauto. Qed.
-
-    Lemma approximates_pure {AT A} `{Subst AT, Inst AT A} {Γ Σ} (ι : SymInstance Σ) (a : AT Σ) :
-      box approximates ι (dmut_pure (Γ := Γ) a) (scmut_pure (inst ι a)).
-    Proof. Admitted.
-
-    Lemma approximates_fail `{Inst AT A} {D Γ1 Γ2 Σ} func msg data ι s :
-      box approximates ι (@dmut_fail Γ1 Γ2 AT Σ D func msg data) s.
-    Proof. Admitted.
-
-    Lemma approximates_block `{Inst AT A} {Γ1 Γ2 Σ} (ι : SymInstance Σ) :
-      box approximates ι (@dmut_block Γ1 Γ2 AT Σ) (@scmut_block Γ1 Γ2 A).
-    Proof. Admitted.
-
-    Lemma dmut_wp_demonic_binary {Γ1 Γ2 Σ0 A} (m1 m2 : DynamicMutator Γ1 Γ2 A Σ0) (POST : StateProperty Γ2 A Σ0) :
-      forall Σ1 (ζ01 : Sub Σ0 Σ1) pc1 s1,
-        dmut_wp (dmut_demonic_binary m1 m2) POST ζ01 pc1 s1 <->
-        dmut_wp m1 POST ζ01 pc1 s1 /\ dmut_wp m2 POST ζ01 pc1 s1.
-    Proof. unfold dmut_wp, dmut_demonic_binary; cbn; intuition. Qed.
-
-    Lemma dmut_wp_sub_demonic_binary {A Γ1 Γ2 Σ0 Σ1} (ζ01 : Sub Σ0 Σ1) (m1 m2 : DynamicMutator Γ1 Γ2 A Σ0) (POST : StateProperty Γ2 A Σ1) :
-      forall Σ2 (ζ12 : Sub Σ1 Σ2) pc2 s2,
-        dmut_wp (dmut_sub ζ01 (dmut_demonic_binary m1 m2)) POST ζ12 pc2 s2 <->
-        dmut_wp (dmut_sub ζ01 m1) POST ζ12 pc2 s2 /\ dmut_wp (dmut_sub ζ01 m2) POST ζ12 pc2 s2.
-    Proof. unfold dmut_wp, dmut_demonic_binary; cbn; intuition. Qed.
-
-    Lemma approximates_demonic_binary {Γ1 Γ2 Σ} (ι : SymInstance Σ)
-          (dm1 dm2 : DynamicMutator Γ1 Γ2 Unit Σ) (sm1 sm2 : SCMut Γ1 Γ2 unit) :
-      box approximates ι dm1 sm1 ->
-      box approximates ι dm2 sm2 ->
-      box approximates ι (dmut_demonic_binary dm1 dm2) (scmut_demonic_binary sm1 sm2).
-    Proof.
-      (* unfold box. intros H1 H2 Σ1 ζ1 ι1 H__ι. *)
-      (* specialize (H1 Σ1 ζ1 ι1 H__ι). specialize (H2 Σ1 ζ1 ι1 H__ι). *)
-      (* intros pc s1 POST Hwp Hpc. apply dmut_wp_sub_demonic_binary in Hwp. *)
-      (* destruct Hwp as [Hwp1 Hwp2]. *)
-      (* specialize (H1 pc s1 POST Hwp1 Hpc). specialize (H2 pc s1 POST Hwp2 Hpc). *)
-      (* apply scmut_wp_demonic_binary. split; auto. *)
-    Admitted.
-
-    Lemma scmut_wp_angelic {Γ1 Γ2 A B} (sm : B -> SCMut Γ1 Γ2 A) (s__sc : SCState Γ1) (POST : A -> SCState Γ2 -> Prop) :
-      scmut_wp (scmut_angelic sm) POST s__sc <-> exists v, scmut_wp (sm v) POST s__sc.
-    Proof. unfold scmut_wp, scmut_angelic; cbn; intuition. Qed.
-
-    (* Lemma dmut_wp_angelic {A B Γ1 Γ2 Σ0 Σ1} (ζ01 : Sub Σ0 Σ1) (m : B -> DynamicMutator Γ1 Γ2 A Σ0) (POST : StateProperty Γ2 A Σ1) : *)
-    (*   forall pc1 s1, *)
-    (*     dmut_wp (dmut_sub ζ01 (dmut_angelic m)) POST pc1 s1 <-> *)
-    (*     exists b, dmut_wp (dmut_sub ζ01 (m b)) POST pc1 s1. *)
-    (* Proof. Admitted. *)
-
-    Lemma approximates_angelic {AT A BT B} `{InstLaws AT A, InstLaws BT B} {Γ1 Γ2 Σ}
-          (ι : SymInstance Σ)
-      (dm : AT Σ -> DynamicMutator Γ1 Γ2 BT Σ) (dm_dcl : forall a, dmut_dcl (dm a))
-      (sm : A -> SCMut Γ1 Γ2 B)
-      (HYP : forall a, box approximates ι (dm a) (sm (inst ι a))) :
-      box approximates ι
-        (dmut_angelic dm)
-        (scmut_angelic sm).
-    Proof.
-      (* unfold box, approximates, dmut_wp, dmut_sub, dmut_angelic; cbn. *)
-      (* intros * Hrel * Hwp Hpc. specialize (Hwp Σ1 (sub_id _)). *)
-      (* destruct Hwp as [a Hwp]. exists (inst ι a). eapply HYP; eauto. *)
-      (* unfold dmut_wp, dmut_sub. intros. revert Hwp. *)
-      (* rewrite sub_comp_id_right, ?subst_sub_id. *)
-      (* eapply (dm_dcl a) with ζ0; eauto; try easy. *)
-      (* - intros [Σ2 ζ2 pc2 a2 s2] [Σ3 ζ3 pc3 a3 s3] ?. *)
-      (*   rewrite ?sub_comp_id_left. *)
-      (*   now apply stateprop_lift_dcl. *)
-      (* - intros [Σ2 ζ2 pc2 a2 s2] ?. *)
-      (*   rewrite ?sub_comp_id_left. *)
-      (*   now apply stateprop_lift_vac. *)
-      (* - intros [Σ2 ζ2 pc2 a2 s2] []; unfold resultprop_specialize_pc; cbn in *. *)
-      (*   now rewrite sub_comp_id_left in H8. *)
-    Admitted.
-
-    (* Lemma dmut_wp_sub_demonic {A B Γ1 Γ2 Σ0 Σ1} (ζ01 : Sub Σ0 Σ1) (m : B -> DynamicMutator Γ1 Γ2 A Σ0) (POST : StateProperty Γ2 A Σ1) : *)
-    (*   forall pc1 s1, *)
-    (*     dmut_wp (dmut_sub ζ01 (dmut_demonic m)) POST pc1 s1 <-> *)
-    (*     forall b, dmut_wp (dmut_sub ζ01 (m b)) POST pc1 s1. *)
-    (* Proof. unfold dmut_wp, dmut_demonic; cbn; intuition. Qed. *)
-
-    Lemma approximates_demonic {A BT B} `{Inst BT B} {Γ1 Γ2 Σ} (ι : SymInstance Σ)
-      (dm : A -> DynamicMutator Γ1 Γ2 BT Σ)
-      (sm : A -> SCMut Γ1 Γ2 B)
-      (HYP : forall a, box approximates ι (dm a) (sm a)) :
-      box approximates ι
-        (dmut_demonic dm)
-        (scmut_demonic sm).
-    Proof.
-      (* unfold box, approximates. *)
-      (* intros Σ1 ζ01 ι1 Hrel * Hwp Hpc. *)
-      (* apply scmut_wp_demonic. intros a. *)
-      (* rewrite dmut_wp_sub_demonic in Hwp. *)
-      (* specialize (Hwp a). *)
-      (* apply (HYP a) in Hwp; auto. *)
-    Admitted.
-
-    Lemma subst_symbolicstate_produce_chunk {Γ Σ Σ1} (ζ1 : Sub Σ Σ1) (c : Chunk Σ) (s : SymbolicState Γ Σ) :
-      subst ζ1 (symbolicstate_produce_chunk c s) = symbolicstate_produce_chunk (subst ζ1 c) (subst ζ1 s).
-    Proof. now destruct s. Qed.
-
-    (* Lemma dmut_wp_produce_chunk {Γ Σ Σ1} (ζ1 : Sub Σ Σ1) (c : Chunk _) pc (s__sym : SymbolicState Γ _) *)
-    (*       (POST : StateProperty Γ Unit _) (POST_dcl : stateprop_downwards_closed POST) : *)
-    (*   dmut_wp (dmut_sub ζ1 (dmut_produce_chunk c)) POST pc s__sym <-> *)
-    (*   POST Σ1 (sub_id Σ1) pc tt (symbolicstate_produce_chunk (subst ζ1 c) s__sym). *)
-    (* Proof. *)
-    (*   split. *)
-    (*   - intros dwp. *)
-    (*     specialize (dwp Σ1 (sub_id Σ1)). cbn in dwp. *)
-    (*     now rewrite ?sub_comp_id_right, ?subst_sub_id in dwp. *)
-    (*   - intros p Σ2 ζ2. cbn. rewrite subst_sub_comp. revert p. *)
-    (*     apply POST_dcl. apply dmutres_geq_syntactic. *)
-    (*     exists ζ2. *)
-    (*     rewrite sub_comp_id_right, sub_comp_id_left. *)
-    (*     now rewrite subst_symbolicstate_produce_chunk. *)
-    (* Qed. *)
-
-    Lemma dmut_produce_chunk_sound {Γ Σ} (ι : SymInstance Σ) (c : Chunk Σ) :
-      box approximates
-        (Γ1 := Γ) (Γ2 := Γ) ι
-        (dmut_produce_chunk c)
-        (scmut_produce_chunk (inst ι c)).
-    Proof.
-      (* intros ? ? ? <- ? ? ? Hwp Hpc. cbn. *)
-      (* apply dmut_wp_produce_chunk in Hwp. *)
-      (* - specialize (Hwp ι1). inster Hwp by apply syminstance_rel_refl. *)
-      (*   specialize (Hwp Hpc). destruct s__sym as [δ h]; cbn. *)
-      (*   now rewrite <- inst_subst. *)
-      (* - apply stateprop_lift_dcl. *)
-    Admitted.
-
-    (* Lemma dmut_wp_sub {Γ1 Γ2 A Σ0} (d : DynamicMutator Γ1 Γ2 A Σ0) *)
-    (*       (POST : StateProperty Γ2 A Σ0) pc (s : SymbolicState Γ1 Σ0) Σ1 (ζ : Sub Σ0 Σ1) : *)
-    (*     dmut_wp d POST pc s -> *)
-    (*     dmut_wp (dmut_sub ζ d) (stateprop_specialize ζ POST) (subst ζ pc) (subst ζ s). *)
-    (* Proof. *)
-    (*   unfold dmut_sub, dmut_wp. intros * Hpost *. *)
-    (*   specialize (Hpost Σ2 (sub_comp ζ ζ1)). *)
-    (*   rewrite ?subst_sub_comp in Hpost. revert Hpost. *)
-    (*   apply outcome_satisfy_monotonic. clear. intros [Σ3 ζ3 pc3 a3 s3]. *)
-    (*   unfold stateprop_specialize. now rewrite sub_comp_assoc. *)
-    (* Qed. *)
-
-    Opaque subst.
-    Opaque sub_up1.
-    Opaque sub_snoc.
-    Opaque wk1.
-    Opaque SubstEnv.
-
-    Lemma dmut_wp_bind {AT A BT B} {instA : Inst AT A} {instB : Inst BT B} {subB: Subst BT}
-          {Γ1 Γ2 Γ3 Σ0 Σ1} (ζ1 : Sub Σ0 Σ1)
-          (ma : DynamicMutator Γ1 Γ2 AT Σ0)
-          (f : forall Σ', Sub Σ0 Σ' -> AT Σ' -> DynamicMutator Γ2 Γ3 BT Σ')
-          (f_dcl : forall Σ ζ a, dmut_dcl (f Σ ζ a))
-          (POST : StateProperty Γ3 BT Σ1) (POST_dcl : stateprop_downwards_closed POST) :
-      forall Σ2 (ζ12 : Sub Σ1 Σ2) pc2 s2,
-        dmut_wp (dmut_sub ζ1 (dmut_bind ma f)) POST ζ12 pc2 s2 <->
-        dmut_wp
-          (dmut_sub ζ1 ma)
-          (fun Σ2 ζ2 pc2 a2 => dmut_wp (f Σ2 (sub_comp ζ1 ζ2) a2) (stateprop_specialize ζ2 POST) (sub_id _) pc2)
-          ζ12 pc2 s2.
-    Proof.
-      (* unfold DynamicMutator, dmut_bind, dmut_sub, dmut_wp, dmut_dcl in *; cbn; intros pc1 s1. *)
-      (* split; intros H Σ2 ζ2; specialize (H Σ2 ζ2). revert H. *)
-      (* - rewrite outcome_satisfy_bind. apply outcome_satisfy_monotonic. *)
-      (*   intros [Σ3 ζ3 pc3 a3 s3] H Σ4 ζ4. revert H. *)
-      (*   rewrite outcome_satisfy_bind. *)
-      (*   eapply f_dcl. *)
-
-      (* OLD: *)
-      (*   apply (f_wf Σ3 (sub_comp (sub_comp ζ1 ζ2) ζ3) a3 Σ3 Σ4 (sub_id Σ3) ζ4) in H. *)
-      (*   + revert H. rewrite sub_comp_id_left, sub_comp_assoc. *)
-      (*     apply outcome_satisfy_monotonic. *)
-      (*     intros [Σ5 ζ5 b5 s5]. cbn. *)
-      (*     now rewrite <- sub_comp_assoc. *)
-      (*   + revert POST_dcl. clear. intros. *)
-      (*     unfold resultprop_downwards_closed. *)
-      (*     intros [Σ4 ζ4 b4 s4] [Σ5 ζ5 b5 s5] Hgeq. *)
-      (*     cbn. apply POST_dcl. rewrite <- ?sub_comp_assoc. *)
-      (*     revert Hgeq. apply dmutres_geq_sem_pre_comp. *)
-      (* - rewrite outcome_satisfy_bind. revert H. *)
-      (*   apply outcome_satisfy_monotonic. *)
-      (*   intros [Σ3 ζ3 a3 s3] H. specialize (H Σ3 (sub_id _)). *)
-      (*   revert H. rewrite outcome_satisfy_bind, subst_sub_id, sub_comp_assoc. *)
-      (*   apply outcome_satisfy_monotonic. *)
-      (*   intros [Σ4 ζ4 b4 s4]. cbn. *)
-      (*   unfold stateprop_specialize. *)
-      (*   now rewrite sub_comp_id_left, sub_comp_assoc. *)
-    Admitted.
-
-    Lemma inst_snoc_wk1 {Σ2 x τ} {ι0 : SymInstance (Σ2 ▻ (x :: τ))} {ι1} `{Subst AT} {substLawsA : SubstLaws AT} `{Inst AT A} {instLaws : InstLaws AT A} {t : AT Σ2} {v} :
-      syminstance_rel (sub_id Σ2 ► (x :: τ ↦ v)) ι0 ι1 -> inst ι0 (wk1 t) = inst ι1 t.
-    Proof.
-      unfold syminstance_rel.
-      intros; subst ι0.
-      change (wk1 t) with (subst (sub_wk1 (b := x :: τ)) t).
-      rewrite inst_subst.
-      f_equal.
-      rewrite <-inst_subst.
-      change (subst (sub_id Σ2 ► (x :: τ ↦ v)) sub_wk1) with (sub_comp sub_wk1 (sub_id Σ2 ► (x :: τ ↦ v))).
-      rewrite sub_comp_wk1_tail. cbn.
-      now rewrite inst_sub_id.
-    Qed.
-
-    (* Section WpSubFresh. *)
-    (*   Local Transparent wk1 subst. *)
-    (*   Lemma dmut_wp_sub_fresh {Γ Σ0 Σ1 AT A x τ} `{Subst AT, Inst AT A} *)
-    (*         (ζ1 : Sub Σ0 Σ1) *)
-    (*         (d : DynamicMutator Γ Γ AT (Σ0 ▻ (x,τ))%ctx) *)
-    (*         (POST : StateProperty Γ AT Σ1) *)
-    (*         (POST_dcl : stateprop_downwards_closed POST) *)
-    (*         (POST_vac : stateprop_vacuous POST) *)
-    (*         (pc : PathCondition Σ1) *)
-    (*         (s : SymbolicState Γ Σ1) (wfd : dmut_dcl d) : *)
-    (*     dmut_wp (dmut_sub ζ1 (dmut_fresh x τ d)) POST pc s <-> *)
-    (*     dmut_wp (dmut_sub (sub_up1 ζ1) d) (stateprop_specialize sub_wk1 POST) (subst sub_wk1 pc) (subst sub_wk1 s). *)
-    (*   Proof. *)
-    (*     unfold dmut_wp, dmut_sub, dmut_fresh. cbn; split; intros HYP Σ2 ζ2. *)
-    (*     - dependent elimination ζ2 as [@env_snoc Σ1 ζ2 _ v]; cbn in v. *)
-    (*       rewrite <- ?subst_sub_comp, ?sub_comp_wk1_tail; cbn. *)
-    (*       specialize (HYP Σ2 ζ2). *)
-    (*       rewrite outcome_satisfy_map in HYP; cbn in *. *)
-    (*       refine (wfd _ Σ2 _ _ _ (env_snoc (sub_id _) (_,τ) v) _ _ _ _ _ _ _ _ _ _ _ HYP); clear wfd HYP; unfold wk1. *)
-    (*       + rewrite <-subst_sub_comp, sub_comp_wk1_tail; cbn. *)
-    (*         now rewrite subst_sub_id. *)
-    (*       + rewrite <-subst_sub_comp, sub_comp_wk1_tail; cbn. *)
-    (*         now rewrite subst_sub_id. *)
-    (*       + change (subst _ (sub_comp _ sub_wk1 ► (x :: τ ↦ _))) with *)
-    (*             (sub_comp (sub_comp (sub_comp ζ1 ζ2) sub_wk1) (sub_id Σ2 ► (fresh Σ2 (Some x) :: τ ↦ v)) ► (x :: τ ↦ v)). *)
-    (*         rewrite <-sub_snoc_comp, sub_comp_assoc, sub_comp_wk1_tail; cbn. *)
-    (*         now rewrite sub_comp_id_right. *)
-    (*       + revert POST_dcl. clear. intros. *)
-    (*         unfold resultprop_downwards_closed. *)
-    (*         intros [Σ3 ζ3 pc3 a3 s3] [Σ4 ζ4 pc4 a4 s4] Hgeq. *)
-    (*         cbn. apply POST_dcl. *)
-    (*         rewrite <- ?sub_comp_assoc. *)
-    (*         revert Hgeq. exact (dmutres_geq_pre_comp _ _ (sub_comp ζ2 sub_wk1)). *)
-    (*       + unfold resultprop_vacuous. *)
-    (*         intros [Σ3 ζ3 pc3 a3 s3]. *)
-    (*         cbn. *)
-    (*         eapply POST_vac. *)
-    (*       + intros [Σ3 ζ3 pc3 a3 s3]. *)
-    (*         unfold resultprop_specialize_pc. cbn. *)
-    (*         intros [geqpc post]. *)
-    (*         rewrite <-(sub_comp_assoc sub_wk1), sub_comp_wk1_tail in post. *)
-    (*         cbn in post. *)
-    (*         rewrite sub_comp_id_left in post. *)
-    (*         unfold stateprop_specialize. *)
-    (*         now rewrite <-(sub_comp_assoc sub_wk1), sub_comp_wk1_tail. *)
-    (*     - rewrite outcome_satisfy_map. *)
-    (*       specialize (HYP (Σ2 ▻ (x,τ)) (sub_up1 ζ2)). *)
-    (*       rewrite <- ?subst_sub_comp, ?sub_comp_wk1_comm in HYP. *)
-    (*       change (wk1 (b := (x,τ)) (subst ζ2 ?t)) with (subst (sub_wk1 (b := (x,τ))) (subst ζ2 t)). *)
-    (*       rewrite ?sub_up_comp, <- ?subst_sub_comp. *)
-    (*       revert HYP. *)
-    (*       (* apply outcome_satisfy_monotonic. *) *)
-    (*       (* intros [Σ3 ζ3 pc3 a3 s3]. clear. *) *)
-    (*       (* dependent elimination ζ3 as [@env_snoc Σ2 ζ3 _ t]. *) *)
-    (*       (* unfold stateprop_specialize. cbn. *) *)
-    (*       (* now rewrite <- ?sub_comp_assoc, <- sub_comp_wk1_comm. *) *)
-    (*   Admitted. *)
-    (* End WpSubFresh. *)
-
-    (* Lemma dmut_wp_fresh {Γ Σ0 AT A x τ} `{Subst AT, Inst AT A} *)
-    (*       (d : DynamicMutator Γ Γ AT (Σ0 ▻ (x,τ))%ctx) (d_dcl : dmut_dcl d) *)
-    (*       (POST : StateProperty Γ AT Σ0) *)
-    (*       (POST_dcl : stateprop_downwards_closed POST) *)
-    (*       (POST_vac : stateprop_vacuous POST) *)
-    (*       (pc : PathCondition Σ0) (s : SymbolicState Γ Σ0) : *)
-    (*   dmut_wp (dmut_fresh x τ d) POST pc s <-> *)
-    (*   dmut_wp d (stateprop_specialize sub_wk1 POST) (subst sub_wk1 pc) (subst sub_wk1 s). *)
-    (* Proof. *)
-    (*   rewrite <-dmut_wp_sub_id. *)
-    (*   rewrite dmut_wp_sub_fresh; try assumption . *)
-    (*   now rewrite sub_up1_id, dmut_wp_sub_id. *)
-    (* Qed. *)
-
-    Lemma dmut_bind_sound {Γ1 Γ2 Γ3 Σ0 AT A BT B}
-      `{Subst AT, Inst AT A, InstLaws BT B} (ι0 : SymInstance Σ0)
-      (dma : DynamicMutator Γ1 Γ2 AT Σ0) (dm_dcl : dmut_dcl dma)
-      (sma : SCMut Γ1 Γ2 A)
-      (dmf : forall Σ1, Sub Σ0 Σ1 -> AT Σ1 -> DynamicMutator Γ2 Γ3 BT Σ1)
-      (dmf_dcl : dmut_arrow_dcl dmf)
-      (dmf_dcl' : forall (Σ : LCtx) (ζ : Sub Σ0 Σ) (a : AT Σ), dmut_dcl (dmf Σ ζ a))
-      (smf : A -> SCMut Γ2 Γ3 B) :
-      box approximates ι0 dma sma ->
-      (forall Σ1 (ζ1 : Sub Σ0 Σ1) (a1 : AT Σ1) (ι1 : SymInstance Σ1),
-          syminstance_rel ζ1 ι0 ι1 ->
-          box approximates ι1 (dmf Σ1 ζ1 a1) (smf (inst ι1 a1))) ->
-      box approximates ι0 (dmut_bind dma dmf) (scmut_bind sma smf).
-    Proof.
-      (* intros H__a H__f. *)
-      (* intros Σ1 ζ1 ι1 relι1 pc1 s__sym1 POST H__wp Hpc. *)
-      (* apply scmut_wp_bind. revert Hpc. *)
-      (* apply dmut_wp_sub_bind in H__wp; auto using stateprop_lift_dcl. *)
-      (* specialize (H__a Σ1 ζ1 ι1 relι1). *)
-      (* apply H__a. revert H__wp. apply dmut_wp_monotonic. *)
-      (* intros Σ2 ζ2 pc2 a2 s2 Hwp2 ι2 rel12 Hpc2. revert Hpc2. *)
-      (* specialize (H__f Σ2 (sub_comp ζ1 ζ2) a2 ι2). *)
-      (* inster H__f by eapply syminstance_rel_trans; eauto. *)
-      (* apply approximates_proj in H__f. apply H__f. *)
-      (* revert Hwp2. apply dmut_wp_monotonic. *)
-      (* intros Σ3 ζ3 pc3 b3 s__sym3 H__post ι3 rel23 Hpc3. *)
-      (* apply H__post. apply (syminstance_rel_trans rel12 rel23). assumption. *)
-    Admitted.
-
-    Lemma dmut_bind_right_sound {Γ1 Γ2 Γ3 Σ0 AT A BT B}
-      `{Subst AT, Inst AT A, InstLaws BT B} (ι0 : SymInstance Σ0)
-      (dma : DynamicMutator Γ1 Γ2 AT Σ0) (dm_dcl : dmut_dcl dma) (sma : SCMut Γ1 Γ2 A)
-      (dmb : DynamicMutator Γ2 Γ3 BT Σ0) (dmb_dcl : dmut_dcl dmb) (smb : SCMut Γ2 Γ3 B) :
-      box approximates ι0 dma sma ->
-      box approximates ι0 dmb smb ->
-      box approximates ι0 (dmut_bind_right dma dmb) (scmut_bind_right sma smb).
-    Proof.
-    Admitted.
-
-    Lemma dmut_fresh_sound {Γ Σ ς τ} (ι : SymInstance Σ)
-          (dm : DynamicMutator Γ Γ Unit (Σ ▻ (ς,τ))) (dm_dcl : dmut_dcl dm)
-          (sm : Lit τ -> SCMut Γ Γ unit) :
-      (forall v, box approximates (env_snoc ι _ v) dm (sm v)) ->
-      box approximates ι
-        (dmut_fresh ς τ dm)
-        (scmut_demonic sm).
-    Proof.
-      (* intros HYP. unfold box, approximates. *)
-      (* intros * <- pc1 s1 POST Hwp Hpc. *)
-      (* apply scmut_wp_demonic. intros v. *)
-      (* specialize (HYP v (Σ1 ▻ (ς,τ)) (sub_up1 ζ1) (env_snoc ι1 (ς,τ) v)). *)
-      (* inster HYP by apply syminstance_rel_up; auto. *)
-      (* unfold approximates in HYP. *)
-      (* specialize (HYP (subst sub_wk1 pc1) (subst (sub_wk1) s1) POST). *)
-      (* rewrite ?inst_subst, ?inst_sub_wk1 in HYP. apply HYP; auto. *)
-      (* apply dmut_wp_sub_fresh in Hwp; auto. *)
-      (* - revert Hwp. *)
-      (*   apply dmut_wp_monotonic; cbn. *)
-      (*   unfold stateprop_impl, stateprop_specialize, stateprop_lift. *)
-      (*   intros ? ζ * Hpost ι0 rel10. *)
-      (*   dependent elimination ζ as [@env_snoc Σ0 ζ _ t]. *)
-      (*   apply syminstance_rel_snoc in rel10. *)
-      (*   apply Hpost. now rewrite sub_comp_wk1_tail. *)
-      (* - apply stateprop_lift_dcl. *)
-      (* - eapply stateprop_lift_vac. *)
-    Admitted.
-
-    Lemma dmut_wp_assume_formula {Γ Σ0 Σ1} (ζ01 : Sub Σ0 Σ1) (fml : Formula Σ0) (POST : StateProperty Γ Unit Σ1)
-      (POST_dcl : stateprop_downwards_closed POST) (POST_vac : stateprop_vacuous POST) :
-      forall Σ2 (ζ12 : Sub Σ1 Σ2) pc2 s2,
-        dmut_wp (dmut_sub ζ01 (dmut_assume_formula (Γ := Γ) fml)) POST ζ12 pc2 s2 <->
-        POST Σ2 ζ12 (cons (subst (sub_comp ζ01 ζ12) fml) pc2) tt s2.
-    Proof.
-      unfold dmut_wp, dmut_assume_formula, dmut_sub. intros.
-      destruct (try_solve_formula_spec (subst (sub_comp ζ01 ζ12) fml)); cbn in *.
-      destruct a; cbn in *.
-      - rewrite sub_comp_id_right; split; apply POST_dcl; exists (sub_id _);
-          rewrite ?subst_sub_id; intuition.
-        + intros ι Hpc. rewrite inst_pathcondition_cons in Hpc. intuition.
-        + intros ι Hpc. rewrite inst_pathcondition_cons. intuition.
-      - split; auto. intros _.
-        apply POST_vac. intros ι Hpc. rewrite inst_pathcondition_cons in Hpc.
-        specialize (H ι). intuition.
-      - clear H.
-        pose proof (dmutres_assume_formula_spec pc2 (subst (sub_comp ζ01 ζ12) fml) s2).
-        destruct (dmutres_assume_formula pc2 (subst (sub_comp ζ01 ζ12) fml) s2) as [Σ3 ζ23 pc3 [] s3].
-        destruct H as [H1 H2].
-        split; apply POST_dcl.
-        + apply dmutres_geq_pre_comp with _ _ _ ζ12 in H1. cbn - [dmutres_geq] in H1.
-          now rewrite sub_comp_id_right in H1.
-        + apply dmutres_geq_pre_comp with _ _ _ ζ12 in H2. cbn - [dmutres_geq] in H2.
-          now rewrite sub_comp_id_right in H2.
-    Qed.
-
-    Lemma dmut_assume_formula_sound {Γ Σ} (ι : SymInstance Σ) (fml : Formula Σ) :
-      box approximates
-        (Γ1 := Γ) (Γ2 := Γ) ι
-        (dmut_assume_formula fml)
-        (scmut_assume_formula ι fml).
-    Proof.
-      unfold box, approximates.
-      intros * <- ? ? ? ? ? POST -> Hpc Hwp.
-      rewrite dmut_wp_assume_formula in Hwp;
-        [|eapply stateprop_lift_dcl|eapply stateprop_lift_vac].
-      unfold stateprop_lift in Hwp.
-      specialize (Hwp ι0 eq_refl).
-      unfold scmut_wp, scmut_assume_formula. cbn.
-      rewrite subst_sub_comp, inst_pathcondition_cons, ?inst_subst in Hwp.
-      intuition.
-    Qed.
-
-    Lemma dmut_wp_angelic_binary {Γ1 Γ2 AT D} `{Subst AT} {Σ0 Σ1} (ζ01 : Sub Σ0 Σ1) (func msg : string) (data : D)
-          (d1 d2 : DynamicMutator Γ1 Γ2 AT Σ0) :
-      forall Σ2 POST (ζ12 : Sub Σ1 Σ2) pc2 s2,
-        dmut_wp (dmut_sub ζ01 (dmut_angelic_binary d1 d2)) POST ζ12 pc2 s2 <->
-        (dmut_wp (dmut_sub ζ01 d1) POST ζ12 pc2 s2 \/
-         dmut_wp (dmut_sub ζ01 d2) POST ζ12 pc2 s2).
-    Proof.
-      intros POST ζ12 pc2 s2.
-      unfold dmut_wp, dmut_sub, dmut_angelic_binary; cbn.
-      intuition.
-    Qed.
-
-    Lemma dmut_wp_angelic_list {Γ1 Γ2 AT D} `{Subst AT} {Σ0 Σ1} (ζ01 : Sub Σ0 Σ1) (func msg : string) (data : D)
-          (xs : list (DynamicMutator Γ1 Γ2 AT Σ0)) :
-      forall Σ2 POST (ζ12 : Sub Σ1 Σ2) pc2 s2,
-        dmut_wp (dmut_sub ζ01 (dmut_angelic_list func msg data xs)) POST ζ12 pc2 s2 <->
-        (exists d, List.In d xs /\
-                dmut_wp (dmut_sub ζ01 d) POST ζ12 pc2 s2).
-    Proof.
-      revert ζ01.
-      induction xs.
-      - intros ζ01 POST ζ12 pc2 s2; cbn.
-        split.
-        + intros [[ctr] _].
-          admit.
-        + admit.
-      - intros ζ01 Σ2 POST ζ12 pc2 s2; cbn.
-        destruct xs.
-        + split.
-          intros Hwp.
-          exists a; split; eauto.
-          intros [d [[->|[]] Hwp]].
-          eauto.
-        + split.
-          * intros [Hwp|Hwp].
-            exists a. split; eauto.
-            destruct (proj1 (IHxs ζ01 Σ2 POST ζ12 pc2 s2) Hwp) as [d2 [d2InDs Hwp2]].
-            exists d2; eauto.
-          * intros [d0 [[<-|d0InDs] Hwp]].
-            left. exact Hwp.
-            right.
-            eapply (proj2 (IHxs ζ01 Σ2 POST ζ12 pc2 s2)).
-            exists d0; eauto.
-    Admitted.
-
-    (* Lemma dmut_wp_angelic_finite {Γ1 Γ2 AT F} `{finite.Finite F, Subst AT} {Σ0 Σ1} (ζ01 : Sub Σ0 Σ1) (k : F -> DynamicMutator Γ1 Γ2 AT Σ0) : *)
-    (*   forall POST pc s, *)
-    (*     dmut_wp (dmut_sub ζ01 (dmut_angelic_finite F k)) POST pc s <-> *)
-    (*     exists x : F, dmut_wp (dmut_sub ζ01 (k x)) POST pc s. *)
-    (* Proof. *)
-    (*   intros *. unfold dmut_angelic_finite. rewrite dmut_wp_angelic_list. *)
-    (*   split. *)
-    (*   - intros [d [HIn Hwp]]. *)
-    (*     apply List.in_map_iff in HIn. *)
-    (*     destruct HIn as [x [<- ?]]. *)
-    (*     now exists x. *)
-    (*   - intros [x Hwp]. exists (k x). split; auto. *)
-    (*     apply List.in_map. *)
-    (*     apply base.elem_of_list_In. *)
-    (*     apply finite.elem_of_enum. *)
-    (* Qed. *)
-
-    (* Lemma dmut_wp_demonic_finite {Γ1 Γ2 AT F} `{finite.Finite F, Subst AT} {Σ0 Σ1} (ζ01 : Sub Σ0 Σ1) (k : F -> DynamicMutator Γ1 Γ2 AT Σ0) : *)
-    (*   forall POST pc s, *)
-    (*     dmut_wp (dmut_sub ζ01 (dmut_demonic_finite F k)) POST pc s <-> *)
-    (*     forall x : F, dmut_wp (dmut_sub ζ01 (k x)) POST pc s. *)
-    (* Proof. *)
-    (* Admitted. *)
-
-    Opaque dmut_assume_formula.
-
-    Lemma dmut_produce_sound {Γ Σ} (asn : Assertion Σ) (ι : SymInstance Σ) :
-      box approximates
-        (Γ1 := Γ) (Γ2 := Γ) ι
-        (dmut_produce asn)
-        (scmut_produce ι asn).
-    Proof.
-      induction asn; cbn.
-      - apply dmut_assume_formula_sound.
-      - apply dmut_produce_chunk_sound.
-      - apply approximates_demonic_binary.
-        + unfold dmut_assume_term, scmut_assume_term.
-          apply dmut_bind_right_sound; auto_dcl;
-            auto using dmut_assume_formula_sound.
-        + unfold dmut_assume_term, scmut_assume_term.
-          apply dmut_bind_right_sound; auto_dcl;
-            auto using dmut_assume_formula_sound.
-      - (* unfold box, approximates. intros. *)
-        (* rewrite dmut_wp_demonic_finite in H1. *)
-        (* specialize (H1 (inst (T := fun Σ => Term Σ (ty_enum E)) ι k)). *)
-        (* unfold dmut_bind_right in H1. *)
-        (* rewrite dmut_wp_sub_bind in H1. *)
-        (* rewrite dmut_wp_assume_formula in H1. *)
-        (* rewrite sub_comp_id_right in H1. *)
-        (* specialize (H (inst (T := fun Σ => Term Σ (ty_enum E)) ι k)). *)
-        (* unfold box, approximates in H. *)
-        admit.
-      - admit.
-      - admit.
-      - admit.
-      - admit.
-      - admit.
-      - admit.
-      - apply dmut_bind_right_sound; auto_dcl; auto.
-      - apply dmut_fresh_sound; auto_dcl; auto.
-    Admitted.
-
-    Lemma dmut_assert_formula_sound {Γ Σ} (ι : SymInstance Σ) (fml : Formula Σ) :
-      box approximates
-        (Γ1 := Γ) (Γ2 := Γ) ι
-        (dmut_assert_formula fml)
-        (scmut_assert_formula ι fml).
-    Proof. Admitted.
-
-    Lemma dmut_consume_chunk_sound {Γ Σ} (c : Chunk Σ) (ι : SymInstance Σ) :
-      box approximates
-        (Γ1 := Γ) (Γ2 := Γ) ι
-        (dmut_consume_chunk c)
-        (scmut_consume_chunk (inst ι c)).
-    Proof. Admitted.
-
-    Lemma dmut_consume_sound {Γ Σ} (asn : Assertion Σ) (ι : SymInstance Σ) :
-      box approximates
-        (Γ1 := Γ) (Γ2 := Γ) ι
-        (dmut_consume asn)
-        (scmut_consume ι asn).
-    Proof.
-      induction asn; cbn [dmut_consume scmut_consume].
-      - apply dmut_assert_formula_sound.
-      - apply dmut_consume_chunk_sound.
-      - apply approximates_demonic_binary.
-        + apply dmut_bind_right_sound; auto_dcl;
-            unfold dmut_assume_term, scmut_assume_term;
-            auto using dmut_assume_formula_sound.
-        + apply dmut_bind_right_sound; auto_dcl;
-            unfold dmut_assume_term, scmut_assume_term;
-            auto using dmut_assume_formula_sound.
-      - admit.
-      - admit.
-      - admit.
-      - admit.
-      - admit.
-      - admit.
-      - admit.
-      - apply dmut_bind_right_sound; auto_dcl; auto.
-      - apply (approximates_angelic (AT := fun Σ => Term Σ _) (A := Lit _)).
-        intros a; auto_dcl.
-        intros a. apply approximates_sub with (env_snoc ι _ (inst ι a)).
-        apply syminstance_rel_snoc. split.
-        apply syminstance_rel_refl. reflexivity.
-        apply IHasn.
-    Admitted.
-
-    Lemma eval_exp_inst {Γ Σ τ} (ι : SymInstance Σ) (δΓΣ : SymbolicLocalStore Γ Σ) (e : Exp Γ τ) :
-      eval e (inst ι δΓΣ) = inst ι (symbolic_eval_exp δΓΣ e).
-    Proof.
-      induction e; cbn; repeat f_equal; auto.
-      { unfold inst; cbn. now rewrite env_lookup_map. }
-      2: {
-        induction es as [|eb n es IHes]; cbn in *.
-        { reflexivity. }
-        { destruct X as [-> Heqs].
-          change (inst_term ?ι ?t) with (inst ι t).
-          destruct (inst ι (symbolic_eval_exp δΓΣ eb));
-            cbn; f_equal; auto.
-        }
-      }
+      induction e; cbn; f_equal; auto.
+      { now rewrite (subst_lookup xInΓ). }
       all: induction es; cbn in *; destruct_conjs; f_equal; auto.
     Qed.
 
-    Lemma dmut_eval_exp_sound {Γ Σ τ} (e : Exp Γ τ) (ι : SymInstance Σ) :
-      box approximates ι (dmut_eval_exp e) (scmut_eval_exp e).
-    Proof.
-      unfold dmut_eval_exps, scmut_eval_exps, box, approximates, dmut_gets_local, dmut_gets, scmut_gets_local, scmut_state_local, dmut_sub, dmut_wp, scmut_wp, stateprop_lift; cbn.
-      intros * <- * -> Hpc Hwp.
-      rewrite sub_comp_id_right in Hwp.
-      specialize (Hwp ι0 eq_refl Hpc).
-      change (scstate_localstore (inst ι0 s__sym)) with (inst ι0 (scstate_localstore s__sym)).
-      refine (eq_ind _ (fun x => POST x _) Hwp _ _).
-      replace (scstate_localstore (inst ι0 s__sym)) with (inst ι0 (symbolicstate_localstore s__sym));
-        eauto using eval_exp_inst.
-      now destruct s__sym.
-    Qed.
-
-    Lemma dmut_eval_exps_sound {Γ Δ Σ} (es : NamedEnv (Exp Γ) Δ) (ι : SymInstance Σ) :
-      box approximates ι (dmut_eval_exps es) (scmut_eval_exps es).
-    Proof.
-      unfold dmut_eval_exps, scmut_eval_exps, box, approximates, dmut_gets_local, dmut_gets, scmut_gets_local, scmut_state_local, dmut_sub, dmut_wp, scmut_wp, stateprop_lift; cbn.
-      intros * <- * -> Hpc Hwp.
-      rewrite sub_comp_id_right in Hwp.
-      specialize (Hwp ι0 eq_refl Hpc).
-      change (scstate_localstore (inst ι0 s__sym)) with (inst ι0 (scstate_localstore s__sym)).
-      unfold inst, inst_localstore, instantiate_env in Hwp.
-      rewrite env_map_map in Hwp.
-      refine (eq_ind _ (fun x => POST x _) Hwp _ _).
-      eapply env_map_ext.
-      replace (scstate_localstore (inst ι0 s__sym)) with (inst ι0 (symbolicstate_localstore s__sym));
-        eauto using eval_exp_inst.
-      now destruct s__sym.
-    Qed.
-
-    Lemma dmut_state_sound {AT A} `{Inst AT A} {Γ1 Γ2 Σ1} (ι1 : SymInstance Σ1)
-          (f : forall Σ2 (ζ12 : Sub Σ1 Σ2), SymbolicState Γ1 Σ2 -> AT Σ2 * SymbolicState Γ2 Σ2)
-          (g  : SCState Γ1 -> A * SCState Γ2)
-          (fg : forall Σ2 (ζ12 : Sub Σ1 Σ2) (ι2 : SymInstance Σ2) s2,
-              syminstance_rel ζ12 ι1 ι2 ->
-              inst ι2 (f Σ2 ζ12 s2) = g (inst ι2 s2)) :
-      box approximates ι1 (dmut_state f) (scmut_state g).
-    Proof.
-      unfold box, approximates, dmut_state, scmut_state, stateprop_lift, dmut_wp, dmut_sub, scmut_wp; cbn.
-      intros Σ2 ζ12 ι2 <- Σ3 ζ23 pc3 s__sym ι3 POST -> Hpc3 Hf; cbn in *.
-      destruct (f Σ3 (sub_comp ζ12 ζ23) s__sym) eqn:?; cbn in *.
-      rewrite sub_comp_id_right in Hf.
-      pose proof (f_equal (inst ι3) Heqp) as Hinst.
-      rewrite fg in Hinst; auto. rewrite Hinst. cbn.
-      apply Hf; auto.
-      unfold sub_comp, syminstance_rel.
-      now rewrite inst_subst.
-    Qed.
-
-    Lemma dmut_call_sound {Γ Δ τ Σ} (c : SepContract Δ τ) (ts : NamedEnv (Term Σ) Δ) (ι : SymInstance Σ) :
-      box approximates ι (@dmut_call Γ Δ τ Σ c ts) (scmut_call c (inst ι ts)).
-    Proof.
-      destruct c as [Σ__c δ pre result post]; cbn [dmut_call scmut_call].
-      apply approximates_angelic; intros; auto_dcl.
-    Admitted.
-
-    Lemma dmut_exec_sound {Γ Σ σ} (s : Stm Γ σ) (ι : SymInstance Σ) :
-      box approximates ι (dmut_exec s) (scmut_exec s).
-    Proof.
-      induction s; cbn [dmut_exec scmut_exec].
-      - pose proof (approximates_pure (Γ := Γ) (ι := ι) (a := term_lit τ l)).
-        now cbn in H.
-      - apply dmut_eval_exp_sound.
-      - apply dmut_bind_sound; auto_dcl.
-        + admit.
-        + admit.
-        + admit.
-      - admit.
-      - apply dmut_bind_sound; auto_dcl.
-        + admit.
-        + admit.
-        + intros.
-          apply dmut_bind_right_sound.
-          admit.
-          admit.
-          apply dmut_state_sound.
-          { intros ? ? ? [δ h] ?; cbn.
-            f_equal. f_equal.
-            unfold inst; cbn.
-            rewrite env_map_update.
-            rewrite inst_subst.
-            unfold syminstance_rel in *. subst.
-            reflexivity.
-          }
-          apply approximates_pure.
-      - destruct (CEnv f) as [c|] eqn:?.
-        + apply dmut_bind_sound; intros; auto_dcl.
-          apply dmut_eval_exps_sound.
-          apply dmut_call_sound.
-        + admit.
-      - admit.
-      - admit.
-      - admit.
-      - admit.
-      - admit.
-      - apply approximates_block.
-      - admit.
-      - admit.
-      - admit.
-      - admit.
-      - admit.
-      - admit.
-      - admit.
-      - admit.
-      - admit.
-      - apply approximates_fail.
-    Admitted.
-
-    Lemma dmut_leakcheck_sound {Γ Σ} (ι : SymInstance Σ) :
-      box approximates ι (@dmut_leakcheck Γ Σ) (@scmut_leakcheck Γ).
-    Proof.
-      unfold box, approximates, dmut_wp, scmut_wp; cbn; intros.
-      rewrite outcome_satisfy_bind in Hwp.
-      destruct s__sym as [σ []]; cbn in *.
-      - unfold stateprop_lift in Hwp. specialize (Hwp ι0).
-        rewrite ?sub_comp_id_right, subst_sub_id in Hwp.
-        eapply Hwp; eauto.
-      - exact (Hwp _ Hpc).
-    Qed.
-
-    Opaque dmut_consume dmut_exec dmut_leakcheck dmut_produce.
-    Opaque scmut_consume scmut_exec scmut_leakcheck scmut_produce.
-
-    Lemma dmut_contract_sound {Γ τ} (c : SepContract Γ τ) (s : Stm Γ τ) (ι : SymInstance (sep_contract_logic_variables c)) :
-      box approximates ι (@dmut_contract Γ τ c s) (@scmut_contract Γ τ c s ι).
-    Proof.
-      (* unfold dmut_contract, scmut_contract; destruct c as [Σ δ pre result post]; cbn in *. *)
-      (* unfold dmut_bind_right. *)
-      (* apply dmut_bind_sound; intros; auto_dcl. *)
-      (* apply dmut_produce_sound. *)
-      (* eapply approximates_sub; eauto. *)
-      (* apply dmut_bind_sound; intros; auto_dcl. *)
-      (* apply dmut_exec_sound. *)
-      (* apply dmut_bind_sound; intros; auto_dcl. *)
-      (* eapply approximates_sub; eauto. *)
-      (* unfold syminstance_rel in *; subst. rewrite <- H0. *)
-      (* apply dmut_consume_sound. *)
-      (* eapply approximates_sub; eauto. *)
-      (* apply dmut_leakcheck_sound. *)
-    Admitted.
-
-    Opaque scmut_contract dmut_contract.
-
-    Lemma outcome_satisfy_bimap {E F A B : Type} (o : Outcome E A) (f : E -> F) (g : A -> B) Q (P : B -> Prop) :
-      outcome_satisfy (outcome_bimap f g o) Q P <-> outcome_satisfy o (fun e => Q (f e)) (fun a => P (g a)).
-    Proof. induction o; firstorder. Qed.
-
-    Lemma outcome_satisfy_bimonotonic {E A} {P Q : E -> Prop} {R S : A -> Prop} (o : Outcome E A)
-          (hype : forall e, P e -> Q e)
-          (hypa : forall a, R a -> S a) :
-      outcome_satisfy o P R -> outcome_satisfy o Q S.
-    Proof. induction o; firstorder. Qed.
-
-    Lemma symbolic_sound {Γ τ} (c : SepContract Γ τ) (body : Stm Γ τ) :
-      ValidContractDynMut c body ->
-      ValidContractSCMut c body.
-    Proof.
-      (* unfold ValidContractDynMut, ValidContractSCMut, outcome_safe, *)
-      (*   dmut_contract_outcome, semiconcrete_outcome_contract; cbn. *)
-      (* rewrite outcome_satisfy_bimap. intros Hd ι. *)
-      (* pose proof (@dmut_contract_sound _ _ c body ι) as H. apply approximates_proj in H. *)
-      (* specialize (H nil (symbolicstate_initial (sep_contract_localstore c))). *)
-      (* rewrite outcome_satisfy_map. *)
-      (* match goal with *)
-      (* | |- outcome_satisfy ?o ?F ?P => *)
-      (*   change (outcome_satisfy o F (fun r => (fun v s => P (MkSCMutResult v s)) (scmutres_value r) (scmutres_state r))) *)
-      (* end. *)
-      (* apply H; [ idtac | now compute ]. clear H. *)
-      (* match goal with *)
-      (* | H: outcome_satisfy ?o (fun _ : DynamicMutatorError => False) ?P |- _ => *)
-      (*   apply (@outcome_satisfy_bimonotonic _ _ _ contradiction P P) in H; *)
-      (*     auto; try contradiction *)
-      (* end. *)
-      (* intros Σ1 ζ01. revert Hd. *)
-      (* eapply dmut_contract_dcl with ζ01; *)
-      (*   rewrite ?subst_sub_id_right; try easy. *)
-      (* intros [Σ2 ζ12 pc2 [] s2]; unfold stateprop_lift; cbn; auto. *)
-    Admitted.
-
-    Section Leftovers.
-
-      Context `{HL: IHeaplet L} {SLL: ISepLogicLaws L}.
-
-      Definition interpret_heap {Σ} (ι : SymInstance Σ) (h : SymbolicHeap Σ) : L :=
-        List.fold_right (fun c h => ASS.inst_chunk ι c ∧ h) ltrue h.
-
-      Transparent subst SubstEnv.
-      Lemma subst_lookup {Γ Σ Σ' x σ} (xInΓ : (x ∶ σ)%ctx ∈ Γ) (ζ : Sub Σ Σ') (δ : SymbolicLocalStore Γ Σ) :
-        (subst ζ (δ ‼ x)%exp = (subst ζ δ ‼ x)%exp).
-      Proof.
-        unfold subst at 2, subst_localstore, SubstEnv.
-        now rewrite env_lookup_map.
-      Qed.
-
-      Lemma subst_symboliceval {Γ τ Σ Σ'} (e : Exp Γ τ) (ζ : Sub Σ Σ') (δ : SymbolicLocalStore Γ Σ) :
-        subst (T := fun Σ => Term Σ _) ζ (symbolic_eval_exp δ e) = symbolic_eval_exp (subst ζ δ) e.
-      Proof.
-        induction e; cbn; f_equal; auto.
-        { now rewrite (subst_lookup xInΓ). }
-        all: induction es; cbn in *; destruct_conjs; f_equal; auto.
-      Qed.
-
-      Transparent inst instantiate_env.
-
-    End Leftovers.
-
-  End DynMutV1Soundness.
+  End Leftovers.
 
 End Soundness.
